Prove simulation theorem, fix bugs in theorem automation, add automation draft for reals

icing/icing_optimisationsLib.sml
@@ -5,17 +5,11 @@
 structure icing_optimisationsLib =
 struct
 
-open floatToRealProofsTheory source_to_sourceProofsTheory listTheory Portable;
+open floatToRealProofsTheory icing_realIdProofsTheory source_to_sourceProofsTheory
+     listTheory Portable;
 open preamble;
 
 local
-  val empty_plan_correct_thm =
-    let val empty_rw_list_correct = MP (Q.SPEC ‘[]’ lift_rewriteFPexp_correct_list) empty_rw_correct
-    in
-      Q.SPEC ‘[]’ is_rewriteFPexp_correct_lift_perform_rewrites
-      |> (fn th => MP th empty_rw_list_correct)
-    end;
-
   fun mk_single_rewriteFPexp_correct_thm th1 th2 =
     let
       val arglist =
@@ -77,17 +71,17 @@ fun mk_plan_correct_thm plan_list :(term * thm)=
         val dtype_comb = rator p1
        in
         (* Simple case: "Label s" --> can be appended to the correctness theorem *)
-        if (Term.compare(dtype_comb, “Label”) = EQUAL)
+        if (Term.compare(dtype_comb, “source_to_source$Label”) = EQUAL)
         then
           (full_plan,
               MP (Q.SPECL [‘^(rand p1)’, ‘^rec_plan’] is_perform_rewrites_correct_label) rec_thm)
         (* Simple case: "Expected e" --> can be appended to the correctness theorem *)
-        else if (Term.compare(dtype_comb, “Expected”) = EQUAL)
+        else if (Term.compare(dtype_comb, “source_to_source$Expected”) = EQUAL)
         then (full_plan,
               MP (Q.SPECL [‘^(rand p1)’, ‘^rec_plan’] is_perform_rewrites_correct_expected) rec_thm)
         else (* Must be an Apply (path, rws) now *)
         let
-          val _ = if (Term.compare(dtype_comb, “Apply”) <> EQUAL)
+          val _ = if (Term.compare(dtype_comb, “source_to_source$Apply”) <> EQUAL)
                   then raise Feedback.mk_HOL_ERR "" "" "Internal err, expected Apply" else ()
           val (pth, rws) = rand p1 |> dest_pair
           (* corr_thms = list of is_rewriteFPexp_correct theorems *)
@@ -102,7 +96,6 @@ fun mk_plan_correct_thm plan_list :(term * thm)=
                           then raise Feedback.mk_HOL_ERR "" "" "Not enough matching theorems"
                           else raise Feedback.mk_HOL_ERR "" "" "Too many matching theorems"
                       else #1 (#2 (hd datas)))
-
             (* |> (fn datas => if (length datas <> 1) then raise ERR "Too many matching theorems" ""
                             else datas)*)
           (* Join the theorems into a single theorem about each of them*)
@@ -146,74 +139,7 @@ fun mk_plan_correct_thm plan_list :(term * thm)=
     end;
 end;
 
-(*
-local
-  fun mk_single_rewriteFPexp_correct_thm th1 th2 =
-    let
-    val arglist =
-      th1 |> concl
-      |> dest_forall |> snd
-      |> dest_forall |> snd
-      |> dest_forall |> snd
-      |> dest_forall |> snd
-      |> dest_forall |> snd
-      |> rator |> rator |> rator |> rator |> rator |> rand;
-    val arg =
-      th2 |> concl
-      |> dest_forall |> snd
-      |> dest_forall |> snd
-      |> dest_forall |> snd
-      |> dest_forall |> snd
-      |> dest_forall |> snd
-      |> rator |> rator |> rator |> rator |> rator |> rand
-      |> listSyntax.dest_list |> fst |> hd (* TODO: Check length *);
-    in
-    SIMP_RULE std_ss [GSYM AND_IMP_INTRO] rewriteExp_compositional
-    |> SPECL [arglist,arg]
-    |> (fn th => MP th th1)
-    |> (fn th => MP th th2)
-    |> SIMP_RULE std_ss [APPEND]
-    end;
-  fun mk_rewriteFPexp_correct_thm_list thms correctthm =
-  case thms of
-   [] => correctthm
-  | th1::thms =>
-    mk_rewriteFPexp_correct_thm_list thms (mk_single_rewriteFPexp_correct_thm correctthm th1);
-  fun mk_rewriteFPexp_list_correct_thm th1 =
-    let
-    val arglist =
-      th1 |> concl
-      |> dest_forall |> snd
-      |> dest_forall |> snd
-      |> dest_forall |> snd
-      |> dest_forall |> snd
-      |> dest_forall |> snd
-      |> rator |> rator |> rator |> rator |> rator |> rand;
-    in
-      SPEC arglist lift_rewriteFPexp_correct_list
-      |> (fn th => MP th th1)
-    end;
-  fun mk_optimise_correct_thm th1 =
-    let
-    val arglist =
-      th1 |> concl
-      |> dest_forall |> snd
-      |> dest_forall |> snd
-      |> dest_forall |> snd
-      |> dest_forall |> snd
-      |> dest_forall |> snd
-      |> rator |> rator |> rator |> rator |> rator |> rand;
-    in
-      SPEC arglist (GEN_ALL is_optimise_correct_lift)
-      |> (fn th => MP th th1)
-    end;
-in
-  fun mk_opt_correct_thm thms =
-  mk_rewriteFPexp_correct_thm_list (List.rev thms) empty_rw_correct
-  |> mk_rewriteFPexp_list_correct_thm
-  |> mk_optimise_correct_thm
-end;
-
+(** Real-valued identity proof *)
 local
   fun mk_single_real_id_thm th1 th2 =
     let
@@ -260,26 +186,88 @@ local
       SPEC arglist lift_real_id_exp_list_strong
       |> (fn th => MP th th1)
     end;
-  fun mk_real_id_optimise_thm th1 =
+
+(* Automatically prove a is_perform_rewrites_correct theorem for the given plan *)
+fun mk_plan_correct_thm plan_list :(term * thm)=
+  case plan_list of
+    (* Base case: Empty plan -> No plan used in correctness theorem *)
+    [] => (“[]:opt_step list”, is_perform_rewrites_correct_empty_plan)
+  | p1 :: ps => (* Cons case *)
+      let
+        (* Recursive call *)
+        val (rec_plan, rec_thm) = mk_plan_correct_thm ps
+        (* Result plan, used for instantiation of theorems *)
+        val full_plan = Parse.Term ‘^p1 :: ^rec_plan’
+        (* Get the Datatype constructor used, can be "Label", "Expected" or "Apply" *)
+        val dtype_comb = rator p1
+       in
+        (* Simple case: "Label s" --> can be appended to the correctness theorem *)
+        if (Term.compare(dtype_comb, “source_to_source$Label”) = EQUAL)
+        then
+          (full_plan,
+              MP (Q.SPECL [‘^(rand p1)’, ‘^rec_plan’] is_perform_rewrites_correct_label_real_id) rec_thm)
+        (* Simple case: "Expected e" --> can be appended to the correctness theorem *)
+        else if (Term.compare(dtype_comb, “source_to_source$Expected”) = EQUAL)
+        then (full_plan,
+              MP (Q.SPECL [‘^(rand p1)’, ‘^rec_plan’] is_perform_rewrites_correct_expected_real_id) rec_thm)
+        else (* Must be an Apply (path, rws) now *)
+        let
+          val _ = if (Term.compare(dtype_comb, “source_to_source$Apply”) <> EQUAL)
+                  then raise Feedback.mk_HOL_ERR "" "" "Internal err, expected Apply" else ()
+          val (pth, rws) = rand p1 |> dest_pair
+          (* corr_thms = list of is_rewriteFPexp_correct theorems *)
+          val corr_thms:thm list = rand p1
+            |> dest_pair |> #2 (* extract the rewrites *)
+            |> listSyntax.dest_list |> #1
+            |> map (fn t => (t, DB.apropos_in t (DB.thy "icing_realIdProofs"))) (* Look up correctness theorems *)
+            |> map (fn (t, thms) =>
+                (print_term t; print (":\n"); map (fn d => print_thm (#1 (#2 d))) thms; thms))
+            |> map (fn datas => if (length datas <> 1)
+                      then if (length datas = 0)
+                          then raise Feedback.mk_HOL_ERR "" "" "Not enough matching theorems"
+                          else raise Feedback.mk_HOL_ERR "" "" "Too many matching theorems"
+                      else #1 (#2 (hd datas)))
+            (* |> (fn datas => if (length datas <> 1) then raise ERR "Too many matching theorems" ""
+                            else datas)*)
+          (* Join the theorems into a single theorem about each of them*)
+          val all_rewrites_correct_thm = mk_real_id_thm_list corr_thms empty_rw_real_id
+          (* lift the theorem to is_rewriteFPexp_list_correct *)
+          val all_rewrites_list_correct_thm = mk_real_id_list_thm all_rewrites_correct_thm
+          (* Extract argument list from theorem *)
+          val args = all_rewrites_list_correct_thm |> concl
+                           |> dest_forall |> snd |> dest_forall |> snd
+                           |> dest_forall |> snd |> dest_forall |> snd
+                           |> dest_forall |> snd
+                           |> rator |> rator |> rator |> rator |> rator |> rand
+          (* build a single perform_rewrites_correct theorem using modus-ponens *)
+          val perform_rw_correct_thm =
+            MP (Q.SPEC ‘^args’ is_real_id_list_perform_rewrites_lift)
+                 all_rewrites_list_correct_thm
+                 |> Q.SPEC ‘^(rand p1 |> dest_pair |> #1)’
+          (* finally, use the "CONS" theorem for plans to prepend the current Apply node *)
+          val final_perform_rw_thm =
+           let
+            val th1 = MP (Q.SPECL [‘^args’, ‘^(rand p1 |> dest_pair |> #1)’, ‘^rec_plan’]
+                     is_perform_rewrites_correct_cons_real_id)
+                   perform_rw_correct_thm
+                in
+               MP th1 rec_thm end
+        in (full_plan, final_perform_rw_thm)
+        end
+        end;
+  in
+  fun mk_stos_pass_real_id_thm plan_list =
     let
-    val arglist =
-      th1 |> concl
-      |> dest_forall |> snd
-      |> dest_forall |> snd
-      |> dest_forall |> snd
-      |> dest_forall |> snd
-      |> dest_forall |> snd
-      |> rator |> rator |> rator |> rator |> rator |> rand;
-    in
-      SPEC arglist (GEN_ALL is_real_id_list_optimise_lift)
-      |> (fn th => MP th th1)
+      val (thePlan, plan_correct_perform_rewrites) = mk_plan_correct_thm plan_list;
+      val plan_correct_optimise_with_plan =
+        MP (Q.SPEC ‘^thePlan’ is_real_id_perform_rewrites_optimise_with_plan_lift)
+           plan_correct_perform_rewrites
+      val stos_pass_correct_with_plan =
+        MP (Q.SPEC ‘[^thePlan]’ stos_pass_with_plans_real_id)
+          (MP (Q.SPEC ‘^thePlan’ is_optimise_with_plan_correct_sing_real_id)
+              plan_correct_optimise_with_plan)
+    in stos_pass_correct_with_plan
     end;
-in
-  fun mk_real_id_thm thms =
-  mk_real_id_thm_list (List.rev thms) empty_rw_real_id
-  |> mk_real_id_list_thm
-  |> mk_real_id_optimise_thm
 end;
-*)
 
 end
