icing/source_to_sourceProofsScript.sml
@@ -27,8 +27,8 @@ QED
 
 Theorem do_app_fp_inv:
   do_app (refs, ffi) (FP_bop op) [v1; v2] = SOME ((refs2, ffi2), r) ==>
-    ∃ w1 w2.
-      fp_translate v1 = SOME (FP_WordTree w1) ∧ fp_translate v2 = SOME (FP_WordTree w2) ∧
+    ? w1 w2.
+      fp_translate v1 = SOME (FP_WordTree w1) /\ fp_translate v2 = SOME (FP_WordTree w2) /\
       r = Rval (FP_WordTree (fp_bop op w1 w2))
 Proof
   Cases_on `op` \\ every_case_tac \\ fs[do_app_def] \\ rpt (TOP_CASE_TAC \\ fs[])
@@ -42,8 +42,8 @@ Proof
 QED
 
 Definition isRealValuedID_rewriteFPexp_def:
-  isRealValuedID_rewriteFPexp ((s,t):fp_pat#fp_pat) (st1:'a semanticPrimitives$state) st2 env e r ⇔
-  evaluate st1 env [realify (rewriteFPexp [(s,t)] e)] = (st2, Rval [Real r]) ⇒
+  isRealValuedID_rewriteFPexp ((s,t):fp_pat#fp_pat) (st1:'a semanticPrimitives$state) st2 env e r <=>
+  evaluate st1 env [realify (rewriteFPexp [(s,t)] e)] = (st2, Rval [Real r]) ==>
   evaluate st1 env [realify e] = (st2, Rval [Real r])
 End
 
@@ -52,10 +52,10 @@ End
  preserve the exact error, as reordering may change which error is returned *)
 Definition is_rewriteFPexp_correct_def:
   is_rewriteFPexp_correct rws (st1:'a semanticPrimitives$state) st2 env e r =
-    (evaluate st1 env [rewriteFPexp rws e] = (st2, Rval r) ∧
-     st1.fp_state.canOpt = FPScope Opt ∧
-     st1.fp_state.real_sem = F ⇒
-     ∃ fpOpt choices fpOptR choicesR.
+    (evaluate st1 env [rewriteFPexp rws e] = (st2, Rval r) /\
+     st1.fp_state.canOpt = FPScope Opt /\
+     st1.fp_state.real_sem = F ==>
+     ? fpOpt choices fpOptR choicesR.
       evaluate
         (st1 with fp_state := st1.fp_state with
            <| rws := st1.fp_state.rws ++ rws; opts := fpOpt; choices := choices |>) env [e] =
@@ -65,10 +65,10 @@ End
 
 Definition is_rewriteFPexp_list_correct_def:
   is_rewriteFPexp_list_correct rws (st1:'a semanticPrimitives$state) st2 env exps r =
-    (evaluate st1 env (MAP (rewriteFPexp rws) exps) = (st2, Rval r) ∧
-     st1.fp_state.canOpt = FPScope Opt ∧
-     st1.fp_state.real_sem = F ⇒
-     ∃ fpOpt choices fpOptR choicesR.
+    (evaluate st1 env (MAP (rewriteFPexp rws) exps) = (st2, Rval r) /\
+     st1.fp_state.canOpt = FPScope Opt /\
+     st1.fp_state.real_sem = F ==>
+     ? fpOpt choices fpOptR choicesR.
        evaluate
          (st1 with fp_state := st1.fp_state with
             <| rws := st1.fp_state.rws ++ rws; opts := fpOpt; choices := choices |>) env exps =
@@ -77,7 +77,7 @@ Definition is_rewriteFPexp_list_correct_def:
 End
 
 Theorem empty_rw_correct:
-   ∀ (st1 st2:'a semanticPrimitives$state) env e r.
+   ! (st1 st2:'a semanticPrimitives$state) env e r.
      is_rewriteFPexp_correct [] st1 st2 env e r
 Proof
   rpt strip_tac \\ fs[is_rewriteFPexp_correct_def, rewriteFPexp_def]
@@ -97,12 +97,12 @@ Proof
 QED
 
 Theorem rewriteExp_compositional:
-  ∀ rws opt.
-   (∀ (st1 st2:'a semanticPrimitives$state) env e r.
-    is_rewriteFPexp_correct rws st1 st2 env e r) ∧
-   (∀ (st1 st2:'a semanticPrimitives$state) env e r.
-    is_rewriteFPexp_correct [opt] st1 st2 env e r) ⇒
-  ∀ (st1 st2:'a semanticPrimitives$state) env e r.
+  ! rws opt.
+   (! (st1 st2:'a semanticPrimitives$state) env e r.
+    is_rewriteFPexp_correct rws st1 st2 env e r) /\
+   (! (st1 st2:'a semanticPrimitives$state) env e r.
+    is_rewriteFPexp_correct [opt] st1 st2 env e r) ==>
+  ! (st1 st2:'a semanticPrimitives$state) env e r.
     is_rewriteFPexp_correct ([opt] ++ rws) st1 st2 env e r
 Proof
   rw[is_rewriteFPexp_correct_def]
@@ -151,9 +151,9 @@ Proof
 QED
 
 Theorem lift_rewriteFPexp_correct_list_strong:
-  ∀ rws (st1 st2:'a semanticPrimitives$state) env exps r.
-    (∀ (st1 st2: 'a semanticPrimitives$state) env e r.
-      is_rewriteFPexp_correct rws st1 st2 env e r) ⇒
+  ! rws (st1 st2:'a semanticPrimitives$state) env exps r.
+    (! (st1 st2: 'a semanticPrimitives$state) env e r.
+      is_rewriteFPexp_correct rws st1 st2 env e r) ==>
   is_rewriteFPexp_list_correct rws st1 st2 env exps r
 Proof
   Induct_on `exps`
@@ -184,10 +184,10 @@ Proof
 QED
 
 Theorem lift_rewriteFPexp_correct_list:
-  ∀ rws.
-    (∀ (st1 st2: 'a semanticPrimitives$state) env e r.
-      is_rewriteFPexp_correct rws st1 st2 env e r) ⇒
-    ∀ (st1 st2:'a semanticPrimitives$state) env exps r.
+  ! rws.
+    (! (st1 st2: 'a semanticPrimitives$state) env e r.
+      is_rewriteFPexp_correct rws st1 st2 env e r) ==>
+    ! (st1 st2:'a semanticPrimitives$state) env exps r.
     is_rewriteFPexp_list_correct rws st1 st2 env exps r
 Proof
   rpt strip_tac \\ drule lift_rewriteFPexp_correct_list_strong
@@ -197,12 +197,12 @@ QED
 Definition is_optimise_with_plan_correct_def:
   is_optimise_with_plan_correct plan (st1:'a semanticPrimitives$state) st2 env cfg exps r =
   (evaluate st1 env
-   (MAP (λ e. FST (optimise_with_plan cfg plan e)) exps) = (st2, Rval r) ∧
-   (cfg.canOpt ⇔ st1.fp_state.canOpt = FPScope Opt) ∧
-   st1.fp_state.canOpt ≠ Strict ∧
-   (~ st1.fp_state.real_sem) ⇒
+   (MAP (λ e. FST (optimise_with_plan cfg plan e)) exps) = (st2, Rval r) /\
+   (cfg.canOpt <=> st1.fp_state.canOpt = FPScope Opt) /\
+   st1.fp_state.canOpt <> Strict /\
+   (~ st1.fp_state.real_sem) ==>
    let theRws = FLAT (MAP (λ x. case x of |Apply (_, rws) => rws |_ => []) plan) in
-   ∃ fpOpt choices fpOptR choicesR.
+   ? fpOpt choices fpOptR choicesR.
      evaluate (st1 with fp_state := st1.fp_state with
                                        <| rws := st1.fp_state.rws ++ theRws;
                                           opts := fpOpt; choices := choices |>) env exps =
@@ -218,13 +218,13 @@ Proof
 QED
 
 Theorem optimise_with_plan_empty_sing:
-  ∀ cfg e. optimise_with_plan cfg [] e = (e, Success)
+  ! cfg e. optimise_with_plan cfg [] e = (e, Success)
 Proof
   fs[optimise_with_plan_def]
 QED
 
 Theorem optimise_with_plan_empty:
-  ∀ exps cfg. MAP (λ e. FST (optimise_with_plan cfg [] e)) exps = exps
+  ! exps cfg. MAP (λ e. FST (optimise_with_plan cfg [] e)) exps = exps
 Proof
   Induct_on ‘exps’ \\ rpt strip_tac
   >- (EVAL_TAC)
@@ -232,14 +232,14 @@ Proof
 QED
 
 Theorem optimise_with_plan_pat_empty:
-  ∀ pl cfg. MAP (λ (p,e). (p, FST (optimise_with_plan cfg [] e))) pl = pl
+  ! pl cfg. MAP (λ (p,e). (p, FST (optimise_with_plan cfg [] e))) pl = pl
 Proof
   Induct_on ‘pl’ \\ rpt strip_tac >- (EVAL_TAC)
   \\ fs[] \\ Cases_on ‘h’ \\ fs[optimise_with_plan_empty_sing]
 QED
 
 Theorem fpState_upd_id:
-  ∀ s.
+  ! s.
     s with fp_state :=
       s.fp_state with <| rws := s.fp_state.rws; opts := s.fp_state.opts |> = s
 Proof
@@ -251,24 +251,24 @@ Proof
 QED
 
 Triviality MAP_MAP_triple:
-  ∀ l f. MAP (λ (x,y,z). x) (MAP (λ (s1,s2,e). (s1,s2,f e)) l) = MAP (λ (x,y,z). x) l
+  ! l f. MAP (λ (x,y,z). x) (MAP (λ (s1,s2,e). (s1,s2,f e)) l) = MAP (λ (x,y,z). x) l
 Proof
   Induct_on ‘l’ \\ fs[] \\ rpt strip_tac
   \\ Cases_on ‘h’ \\ fs[] \\ Cases_on ‘r’ \\ fs[]
 QED
 
 Theorem MEM_for_all_MAPi:
-  ∀ (P: α -> α -> bool) (f: α -> α) (g: α -> α) l l'.
-    (∀x. MEM x l ⇒ P (f x) x) ∧ (∀x. P (g x) x) ⇒
-    MAPi (λn e. if n = i then (f e) else (g e)) l = l' ⇒
-    (∀i. (i: num) < LENGTH l ⇒ P (EL i l') (EL i l))
+  ! (P: 'a -> 'a -> bool) (f: 'a -> 'a) (g: 'a -> 'a) l l'.
+    (!x. MEM x l ==> P (f x) x) /\ (!x. P (g x) x) ==>
+    MAPi (λn e. if n = i then (f e) else (g e)) l = l' ==>
+    (!i. (i: num) < LENGTH l ==> P (EL i l') (EL i l))
 Proof
   rpt strip_tac
   \\ imp_res_tac (INST_TYPE[alpha |-> beta] EL_MAPi)
-  \\ pop_assum ( Q.ISPEC_THEN ‘(λ (n :num) (e :α). if n = (i :num) then ((f :α -> α) e) else (g :α -> α) e): num -> α -> α’ strip_assume_tac )
+  \\ pop_assum ( Q.ISPEC_THEN ‘(λ (n :num) (e :'a). if n = (i :num) then ((f :'a -> 'a) e) else (g :'a -> 'a) e): num -> 'a -> 'a’ strip_assume_tac )
   \\ fs[EVAL “(λn e. if n = i then f e else g e) i' (EL i' l)”]
   \\ Cases_on ‘i = i'’ \\ rveq  \\ fs[]
-  \\ qpat_x_assum ‘∀ x. MEM x l ⇒ P (f x) x’ (qspec_then ‘(EL i l)’ assume_tac)
+  \\ qpat_x_assum ‘! x. MEM x l ==> P (f x) x’ (qspec_then ‘(EL i l)’ assume_tac)
   \\ Q.ISPECL_THEN [‘l’, ‘(EL i l)’] strip_assume_tac MEM_EL
   \\ last_assum ( (assume_tac o snd) o EQ_IMP_RULE ) \\ fs[]
   \\ ‘EL i l = EL i l’ by fs[]
@@ -278,7 +278,7 @@ Proof
 QED
 
 Theorem MAPi_EL_nested:
-  ∀ l n. n < LENGTH l ⇒ EL n (MAPi (λ n e. (n, e)) l) = EL n (MAPi (λ n e. (n, (EL n l))) l)
+  ! l n. n < LENGTH l ==> EL n (MAPi (λ n e. (n, e)) l) = EL n (MAPi (λ n e. (n, (EL n l))) l)
 Proof
   rpt strip_tac
   \\ qspecl_then [‘(λ n e. (n, e))’, ‘n’, ‘l’] imp_res_tac EL_MAPi
@@ -287,7 +287,7 @@ Proof
 QED
 
 Theorem MAPi_EL_no_fun:
-  ∀ l. MAPi (λ n e. (n, e)) l = MAPi (λ n e. (n, (EL n l))) l
+  ! l. MAPi (λ n e. (n, e)) l = MAPi (λ n e. (n, (EL n l))) l
 Proof
   rpt strip_tac
   \\ qspecl_then [‘MAPi (λ n e. (n, e)) l’, ‘MAPi (λ n e. (n, (EL n l))) l’] strip_assume_tac LIST_EQ
@@ -296,7 +296,7 @@ Proof
 QED
 
 Theorem MAPi_EL_list_quant:
-  ∀ f l. MAPi (λ n e. f n e) l = MAPi (λ n e. f n (EL n l)) l
+  ! f l. MAPi (λ n e. f n e) l = MAPi (λ n e. f n (EL n l)) l
 Proof
   rpt strip_tac
   \\ qspecl_then [‘MAPi (λ n e. f n e) l’, ‘MAPi (λ n e. f n (EL n l)) l’] strip_assume_tac LIST_EQ
@@ -311,7 +311,7 @@ Proof
 QED
 
 Theorem MAPi_same_EL_quant:
-  ∀ exps. MAPi (λ n e. (EL n exps)) exps = exps
+  ! exps. MAPi (λ n e. (EL n exps)) exps = exps
 Proof
   strip_tac
   \\ qspecl_then [‘λ n e. e’, ‘exps’] assume_tac MAPi_EL_list_quant
@@ -329,7 +329,7 @@ val rewrites_no_effect =
   “λ cfg path plan e. perform_rewrites cfg path plan e = e”
 in
 Theorem perform_rewrites_no_plan_same:
-  ∀ cfg path plan e. plan = [] ⇒ ^rewrites_no_effect cfg path plan e
+  ! cfg path plan e. plan = [] ==> ^rewrites_no_effect cfg path plan e
 Proof
   ho_match_mp_tac perform_rewrites_ind
   \\ fs[perform_rewrites_def]
@@ -349,14 +349,14 @@ Proof
   \\ Cases_on ‘x = i’
   \\ fs[]
   \\ TRY (
-    qpat_x_assum ‘∀e. MEM e exps ⇒ _’ (qspec_then ‘EL i exps’ assume_tac)
+    qpat_x_assum ‘!e. MEM e exps ==> _’ (qspec_then ‘EL i exps’ assume_tac)
     \\ fs[MEM_EL]
     \\ pop_assum irule
     \\ qexists_tac ‘i’ \\ fs[]
     )
   \\ TRY (
     Cases_on ‘EL i pes’ \\ fs[]
-    \\ qpat_x_assum ‘∀ p e. MEM (p, e) pes ⇒ _’ (qspecl_then [‘q’, ‘r’] assume_tac)
+    \\ qpat_x_assum ‘! p e. MEM (p, e) pes ==> _’ (qspecl_then [‘q’, ‘r’] assume_tac)
     \\ fs[MEM_EL]
     \\ pop_assum irule
     \\ qexists_tac ‘i’ \\ fs[]
@@ -376,19 +376,19 @@ Proof
 QED
 
 Theorem enumerate_append:
-  ∀ l l' n. enumerate n (l ++ l') = (enumerate n l) ++ (enumerate (n + LENGTH l) l')
+  ! l l' n. enumerate n (l ++ l') = (enumerate n l) ++ (enumerate (n + LENGTH l) l')
 Proof
   Induct_on ‘l'’ \\ fs[miscTheory.enumerate_def]
   \\ Induct_on ‘l’ \\ fs[miscTheory.enumerate_def]
 QED
 
 Definition is_perform_rewrites_correct_def:
-  is_perform_rewrites_correct rws (st1:'a semanticPrimitives$state) st2 env cfg e r path ⇔
-    evaluate st1 env [perform_rewrites cfg path rws e] = (st2, Rval r) ∧
-    (cfg.canOpt ⇔ st1.fp_state.canOpt = FPScope Opt) ∧
-    st1.fp_state.canOpt ≠ Strict ∧
-    (~ st1.fp_state.real_sem) ⇒
-    ∃ fpOpt choices fpOptR choicesR.
+  is_perform_rewrites_correct rws (st1:'a semanticPrimitives$state) st2 env cfg e r path <=>
+    evaluate st1 env [perform_rewrites cfg path rws e] = (st2, Rval r) /\
+    (cfg.canOpt <=> st1.fp_state.canOpt = FPScope Opt) /\
+    st1.fp_state.canOpt <> Strict /\
+    (~ st1.fp_state.real_sem) ==>
+    ? fpOpt choices fpOptR choicesR.
       evaluate (st1 with fp_state :=
                   st1.fp_state with
                      <| rws := st1.fp_state.rws ++ rws;
@@ -406,14 +406,14 @@ local
   (* exp goal *)
   val P0 =
   “λ (e:ast$exp).
-     ∀ (st1: 'a semanticPrimitives$state) st2 env cfg rws r path.
-     (∀ (st1:'a semanticPrimitives$state) st2 env exps r.
-       is_rewriteFPexp_list_correct rws st1 st2 env exps r) ∧
-     (cfg.canOpt ⇔ st1.fp_state.canOpt = FPScope Opt) ∧
-     st1.fp_state.canOpt ≠ Strict ∧
-     ~st1.fp_state.real_sem ∧
-     evaluate st1 env [perform_rewrites (cfg with optimisations := rws) path rws e] = (st2, Rval r) ⇒
-    ∃ fpOpt choices fpOptR choicesR.
+     ! (st1: 'a semanticPrimitives$state) st2 env cfg rws r path.
+     (! (st1:'a semanticPrimitives$state) st2 env exps r.
+       is_rewriteFPexp_list_correct rws st1 st2 env exps r) /\
+     (cfg.canOpt <=> st1.fp_state.canOpt = FPScope Opt) /\
+     st1.fp_state.canOpt <> Strict /\
+     ~st1.fp_state.real_sem /\
+     evaluate st1 env [perform_rewrites cfg path rws e] = (st2, Rval r) ==>
+    ? fpOpt choices fpOptR choicesR.
       evaluate (st1 with fp_state := st1.fp_state with
                 <| rws := st1.fp_state.rws ++ rws; opts := fpOpt; choices := choices |>) env [e]=
         (st2 with fp_state := st2.fp_state with
@@ -427,23 +427,23 @@ local
   (* Letrec goal *)
   val P1 =
   Parse.Term (‘λ (l:(string # string # exp) list).
-  ∀ p. MEM p l ⇒ ^P2 p’)
+  ! p. MEM p l ==> ^P2 p’)
   (* P5: pat * exp -> bool *)
   val P5 =
   Parse.Term (‘λ (p:pat, e). ^P0 e’)
   (* P3: pat * exp list -> bool *)
   val P3 =
   Parse.Term (‘λ (l:(pat # exp) list).
-     ∀ (st1: 'a semanticPrimitives$state) st2 env cfg rws r v err_v path i.
-     (∀ (st1:'a semanticPrimitives$state) st2 env exps r.
-        is_rewriteFPexp_list_correct rws st1 st2 env exps r) ∧
-     (cfg.canOpt ⇔ st1.fp_state.canOpt = FPScope Opt) ∧
-     st1.fp_state.canOpt ≠ Strict ∧
-     ~st1.fp_state.real_sem ∧
+     ! (st1: 'a semanticPrimitives$state) st2 env cfg rws r v err_v path i.
+     (! (st1:'a semanticPrimitives$state) st2 env exps r.
+        is_rewriteFPexp_list_correct rws st1 st2 env exps r) /\
+     (cfg.canOpt <=> st1.fp_state.canOpt = FPScope Opt) /\
+     st1.fp_state.canOpt <> Strict /\
+     ~st1.fp_state.real_sem /\
      evaluate_match st1 env v (MAPi (λ n (p,e). if (n = i) then
-                                                  (p, perform_rewrites (cfg with optimisations := rws) path rws e)
-                                                else (p, e)) l) err_v = (st2, Rval r) ⇒
-     ∃ fpOpt choices fpOptR choicesR.
+                                                  (p, perform_rewrites cfg path rws e)
+                                                else (p, e)) l) err_v = (st2, Rval r) ==>
+     ? fpOpt choices fpOptR choicesR.
        evaluate_match
          (st1 with fp_state := st1.fp_state with <| rws := st1.fp_state.rws ++ rws; opts := fpOpt; choices := choices |>)
          env v l err_v =
@@ -451,7 +451,7 @@ local
            <| rws := st2.fp_state.rws ++ rws; opts := fpOptR; choices := choicesR |>, Rval r)’);
   (* P6: exp list -> bool *)
   val P6 =
-    Parse.Term (‘λ (es:ast$exp list). ∀ e. MEM e es ⇒ ^P0 e’);
+    Parse.Term (‘λ (es:ast$exp list). ! e. MEM e es ==> ^P0 e’);
   val ind_thm =
     astTheory.exp_induction |> SPEC P0 |> SPEC P1 |> SPEC P2 |> SPEC P3
     |> SPEC P4 |> SPEC P5 |> SPEC P6;
@@ -483,18 +483,18 @@ val no_change_tac = fn t =>
    \\ fs[semState_comp_eq, fpState_component_equality]);
 
 Triviality lift_P6_perform_rws_REVERSE:
-  ∀ es.
-    ^P6 es ⇒
-    ∀ (st1: 'a semanticPrimitives$state) st2 env cfg rws r path i m.
-    (∀ (st1:'a semanticPrimitives$state) st2 env exps r.
-       is_rewriteFPexp_list_correct rws st1 st2 env exps r) ∧
-    (cfg.canOpt ⇔ st1.fp_state.canOpt = FPScope Opt) ∧
-    st1.fp_state.canOpt ≠ Strict ∧
-    ~st1.fp_state.real_sem ∧
+  ! es.
+    ^P6 es ==>
+    ! (st1: 'a semanticPrimitives$state) st2 env cfg rws r path i m.
+    (! (st1:'a semanticPrimitives$state) st2 env exps r.
+       is_rewriteFPexp_list_correct rws st1 st2 env exps r) /\
+    (cfg.canOpt <=> st1.fp_state.canOpt = FPScope Opt) /\
+    st1.fp_state.canOpt <> Strict /\
+    ~st1.fp_state.real_sem /\
     evaluate st1 env (REVERSE (MAP (λ (n, e). if (n = i) then
-                                     perform_rewrites (cfg with optimisations := rws) path rws e
-                                   else e) (enumerate m es))) = (st2, Rval r) ⇒
-    ∃ fpOpt choices fpOptR choicesR.
+                                     perform_rewrites cfg path rws e
+                                   else e) (enumerate m es))) = (st2, Rval r) ==>
+    ? fpOpt choices fpOptR choicesR.
       evaluate
         (st1 with fp_state := st1.fp_state with <| rws := st1.fp_state.rws ++ rws; opts := fpOpt; choices := choices |>)
         env (REVERSE es) =
@@ -509,15 +509,15 @@ Proof
   \\ fs[evaluate_append]
   \\ qpat_x_assum ‘case evaluate _ _ _ of _ => _’ (assume_tac o SIMP_RULE bool_ss [CaseEq"prod", CaseEq"result"])
   \\ fs[] \\ rveq
-  \\ ‘∀e. MEM e es ⇒
-          ∀(st1 :α semanticPrimitives$state) (st2 :α semanticPrimitives$state) env cfg rws r path.
-            (∀ (st1:'a semanticPrimitives$state) st2 env exps r.
-               is_rewriteFPexp_list_correct rws st1 st2 env exps r)  ∧
-            (cfg.canOpt ⇔ st1.fp_state.canOpt = FPScope Opt) ∧
-            st1.fp_state.canOpt ≠ Strict ∧ ~st1.fp_state.real_sem ∧
+  \\ ‘!e. MEM e es ==>
+          !(st1 :'a semanticPrimitives$state) (st2 :'a semanticPrimitives$state) env cfg rws r path.
+            (! (st1:'a semanticPrimitives$state) st2 env exps r.
+               is_rewriteFPexp_list_correct rws st1 st2 env exps r)  /\
+            (cfg.canOpt <=> st1.fp_state.canOpt = FPScope Opt) /\
+            st1.fp_state.canOpt <> Strict /\ ~st1.fp_state.real_sem /\
             evaluate st1 env
-                     [perform_rewrites (cfg with optimisations := rws) path rws e] = (st2,Rval r) ⇒
-            ∃fpOpt choices fpOptR choicesR.
+                     [perform_rewrites cfg path rws e] = (st2,Rval r) ==>
+            ?fpOpt choices fpOptR choicesR.
               evaluate
               (st1 with
                fp_state :=
@@ -530,22 +530,22 @@ Proof
                   <|rws := st2.fp_state.rws ++ rws; opts := fpOptR;
                     choices := choicesR|>,Rval r)’ by (
     rpt strip_tac
-    \\ qpat_x_assum ‘∀e. e = h ∨ MEM e es ⇒ _’ (qspec_then ‘e’ strip_assume_tac)
+    \\ qpat_x_assum ‘!e. e = h \/ MEM e es ==> _’ (qspec_then ‘e’ strip_assume_tac)
     \\ rfs[] \\ pop_assum (qspecl_then [‘st1'’, ‘st2’, ‘env'’, ‘cfg'’, ‘rws'’, ‘r’, ‘path'’] strip_assume_tac)
     \\ rfs[] \\ qexistsl_tac [‘fpOpt’, ‘choices’, ‘fpOptR’, ‘choicesR’] \\ fs[]
     )
-  \\ qpat_x_assum ‘(∀e. MEM e es ⇒ _) ⇒ _’ drule
+  \\ qpat_x_assum ‘(!e. MEM e es ==> _) ==> _’ drule
   \\ disch_then (qspecl_then [‘st1’, ‘s'’, ‘env’, ‘cfg’, ‘rws’, ‘vs’, ‘path’, ‘i’, ‘m + 1’] strip_assume_tac)
   \\ rfs[]
   \\ Cases_on ‘m = i’ \\ fs[] \\ rveq
   >- (
-  qpat_x_assum ‘∀e. e = h ∨ MEM e es ⇒ _’ (qspec_then ‘h’ strip_assume_tac) \\ fs[]
+  qpat_x_assum ‘!e. e = h \/ MEM e es ==> _’ (qspec_then ‘h’ strip_assume_tac) \\ fs[]
   \\ pop_assum (qspecl_then [‘s'’, ‘s''’, ‘env’, ‘cfg’, ‘rws’, ‘vs'’, ‘path’] strip_assume_tac)
-  \\ ‘(cfg.canOpt ⇔ s'.fp_state.canOpt = FPScope Opt) ∧ s'.fp_state.canOpt ≠ Strict ∧
+  \\ ‘(cfg.canOpt <=> s'.fp_state.canOpt = FPScope Opt) /\ s'.fp_state.canOpt <> Strict /\
       ~s'.fp_state.real_sem’ by (imp_res_tac evaluate_fp_opts_inv \\ fs[]) \\ fs[]
-  \\ qpat_x_assum ‘_ ∧ evaluate _ _ [perform_rewrites _ _ _ _] = _ ⇒ _’ imp_res_tac
+  \\ qpat_x_assum ‘_ /\ evaluate _ _ [perform_rewrites _ _ _ _] = _ ==> _’ imp_res_tac
   \\ optUntil_tac ‘evaluate _ _ (REVERSE es) = _’ ‘fpOpt'’
-  \\ qexistsl_tac [‘optUntil (choicesR − choices) fpOpt fpOpt'’, ‘choices’] \\ fs[]
+  \\ qexistsl_tac [‘optUntil (choicesR - choices) fpOpt fpOpt'’, ‘choices’] \\ fs[]
   \\ ntac 2 (pop_assum kall_tac)
   \\ drule (CONJUNCT1 evaluate_add_choices)
   \\ disch_then (qspec_then ‘choicesR’ strip_assume_tac)
@@ -555,7 +555,7 @@ Proof
   qpat_x_assum ‘evaluate _ _ [h] = _’ (mp_then Any assume_tac (prep (CONJUNCT1 evaluate_fp_rws_append)))
   \\ pop_assum (qspecl_then [‘rws’, ‘s''.fp_state.opts’] strip_assume_tac)
   \\ optUntil_tac ‘evaluate _ _ (REVERSE es) = _’ ‘fpOpt'’
-  \\ qexistsl_tac [‘optUntil (choicesR − choices) fpOpt fpOpt'’, ‘choices’] \\ fs[]
+  \\ qexistsl_tac [‘optUntil (choicesR - choices) fpOpt fpOpt'’, ‘choices’] \\ fs[]
   \\ pop_assum kall_tac
   \\ drule (CONJUNCT1 evaluate_add_choices)
   \\ disch_then (qspec_then ‘choicesR’ strip_assume_tac)
@@ -564,18 +564,18 @@ Proof
 QED
 
 Triviality lift_P6_perform_rws:
-  ∀ es.
-    ^P6 es ⇒
-    ∀ (st1: 'a semanticPrimitives$state) st2 env cfg rws r path i m.
-    (∀ (st1:'a semanticPrimitives$state) st2 env exps r.
-       is_rewriteFPexp_list_correct rws st1 st2 env exps r) ∧
-    (cfg.canOpt ⇔ st1.fp_state.canOpt = FPScope Opt) ∧
-    st1.fp_state.canOpt ≠ Strict ∧
-    ~st1.fp_state.real_sem ∧
+  ! es.
+    ^P6 es ==>
+    ! (st1: 'a semanticPrimitives$state) st2 env cfg rws r path i m.
+    (! (st1:'a semanticPrimitives$state) st2 env exps r.
+       is_rewriteFPexp_list_correct rws st1 st2 env exps r) /\
+    (cfg.canOpt <=> st1.fp_state.canOpt = FPScope Opt) /\
+    st1.fp_state.canOpt <> Strict /\
+    ~st1.fp_state.real_sem /\
     evaluate st1 env (MAP (λ (n, e). if (n = i) then
-                                     perform_rewrites (cfg with optimisations := rws) path rws e
-                                   else e) (enumerate m es)) = (st2, Rval r) ⇒
-    ∃ fpOpt choices fpOptR choicesR.
+                                     perform_rewrites cfg path rws e
+                                   else e) (enumerate m es)) = (st2, Rval r) ==>
+    ? fpOpt choices fpOptR choicesR.
       evaluate
         (st1 with fp_state := st1.fp_state with
                                  <| rws := st1.fp_state.rws ++ rws; opts := fpOpt; choices := choices |>)
@@ -588,12 +588,12 @@ Proof
       \\ fs[semState_comp_eq, fpState_component_equality])
   \\ fs[miscTheory.enumerate_def]
   \\ ‘evaluate st1 env ([(if m = i then
-          perform_rewrites (cfg with optimisations := rws) path rws h
+          perform_rewrites cfg path rws h
         else h)] ++
        MAP
        (λ(n,e).
           if n = i then
-            perform_rewrites (cfg with optimisations := rws) path
+            perform_rewrites cfg path
                              rws e
           else e) (enumerate (m + 1) es)) = (st2, Rval r)’ by fs[]
   \\ fs[evaluate_append]
@@ -603,15 +603,15 @@ Proof
   \\ qpat_x_assum ‘case evaluate _ _ _ of _ => _’ (
                     assume_tac o SIMP_RULE bool_ss [CaseEq"prod", CaseEq"result"])
   \\ fs[] \\ rveq
-  \\ ‘∀e. MEM e es ⇒
-          ∀(st1 :α semanticPrimitives$state) (st2 :α semanticPrimitives$state) env cfg rws r path.
-            (∀ (st1:'a semanticPrimitives$state) st2 env exps r.
-               is_rewriteFPexp_list_correct rws st1 st2 env exps r) ∧
-            (cfg.canOpt ⇔ st1.fp_state.canOpt = FPScope Opt) ∧
-            st1.fp_state.canOpt ≠ Strict ∧ ~st1.fp_state.real_sem ∧
+  \\ ‘!e. MEM e es ==>
+          !(st1 :'a semanticPrimitives$state) (st2 :'a semanticPrimitives$state) env cfg rws r path.
+            (! (st1:'a semanticPrimitives$state) st2 env exps r.
+               is_rewriteFPexp_list_correct rws st1 st2 env exps r) /\
+            (cfg.canOpt <=> st1.fp_state.canOpt = FPScope Opt) /\
+            st1.fp_state.canOpt <> Strict /\ ~st1.fp_state.real_sem /\
             evaluate st1 env
-                     [perform_rewrites (cfg with optimisations := rws) path rws e] = (st2,Rval r) ⇒
-            ∃fpOpt choices fpOptR choicesR.
+                     [perform_rewrites cfg path rws e] = (st2,Rval r) ==>
+            ?fpOpt choices fpOptR choicesR.
               evaluate (st1 with
                         fp_state :=
                         st1.fp_state with
@@ -623,25 +623,25 @@ Proof
                   <|rws := st2.fp_state.rws ++ rws; opts := fpOptR;
                     choices := choicesR|>,Rval r)’ by (
     rpt strip_tac
-    \\ qpat_x_assum ‘∀e. e = h ∨ MEM e es ⇒ _’ (qspec_then ‘e’ strip_assume_tac)
+    \\ qpat_x_assum ‘!e. e = h \/ MEM e es ==> _’ (qspec_then ‘e’ strip_assume_tac)
     \\ rfs[] \\ pop_assum (qspecl_then [‘st1'’, ‘st2’, ‘env'’, ‘cfg'’, ‘rws'’, ‘r’, ‘path'’] strip_assume_tac)
     \\ rfs[] \\ qexistsl_tac [‘fpOpt’, ‘choices’, ‘fpOptR’, ‘choicesR’] \\ fs[]
     )
-  \\ qpat_x_assum ‘(∀e. MEM e es ⇒ _) ⇒ _’ drule
+  \\ qpat_x_assum ‘(!e. MEM e es ==> _) ==> _’ drule
   \\ disch_then (qspecl_then [‘s'’, ‘s''’, ‘env’, ‘cfg’, ‘rws’, ‘vs'’, ‘path’, ‘i’, ‘m + 1’] strip_assume_tac)
   \\ rfs[]
-  \\ ‘(st1.fp_state.canOpt = FPScope Opt ⇔ s'.fp_state.canOpt = FPScope Opt)
-      ∧ s'.fp_state.canOpt ≠ Strict ∧ ~s'.fp_state.real_sem’ by (
+  \\ ‘(st1.fp_state.canOpt = FPScope Opt <=> s'.fp_state.canOpt = FPScope Opt)
+      /\ s'.fp_state.canOpt <> Strict /\ ~s'.fp_state.real_sem’ by (
     imp_res_tac evaluate_fp_opts_inv \\ fs[]
     )
   \\ fs[]
   \\ Cases_on ‘m = i’ \\ fs[] \\ rveq
   >- (
-  qpat_x_assum ‘∀e. e = h ∨ MEM e es ⇒ _’ (qspec_then ‘h’ strip_assume_tac) \\ fs[]
+  qpat_x_assum ‘!e. e = h \/ MEM e es ==> _’ (qspec_then ‘h’ strip_assume_tac) \\ fs[]
   \\ pop_assum (qspecl_then [‘st1’, ‘s'’, ‘env’, ‘cfg’, ‘rws’, ‘vs’, ‘path’] strip_assume_tac)
   \\ rfs[]
   \\ optUntil_tac ‘evaluate _ _ [h] = _’ ‘fpOpt’
-  \\ qexistsl_tac [‘optUntil (choicesR' − choices') fpOpt' fpOpt’, ‘choices'’]
+  \\ qexistsl_tac [‘optUntil (choicesR' - choices') fpOpt' fpOpt’, ‘choices'’]
   \\ fs[semState_comp_eq, fpState_component_equality]
   \\ pop_assum kall_tac
   \\ drule (CONJUNCT1 evaluate_add_choices)
@@ -663,8 +663,8 @@ Proof
 QED
 
 Theorem perform_rewrites_correct:
-  (∀ e. ^P0 e) ∧ (∀ l. ^P1 l) ∧ (∀ p. ^P2 p) ∧ (∀ l. ^P3 l) ∧ (∀ p. ^P4 p)
-  ∧ (∀ p. ^P5 p) ∧ (∀ l. ^P6 l)
+  (! e. ^P0 e) /\ (! l. ^P1 l) /\ (! p. ^P2 p) /\ (! l. ^P3 l) /\ (! p. ^P4 p)
+  /\ (! p. ^P5 p) /\ (! l. ^P6 l)
 Proof
   irule ind_thm \\ rpt strip_tac \\ fs[perform_rewrites_def] \\ rpt strip_tac
   (* Case: If e e0 e1 *)
@@ -679,16 +679,16 @@ Proof
     qpat_x_assum ‘evaluate _ _ [If _ _ _] = _’ (
                    assume_tac o SIMP_RULE bool_ss [evaluate_def, CaseEq"prod", CaseEq"result"])
     \\ fs[] \\ rveq
-    \\ Cases_on ‘do_if (HD v) (perform_rewrites (cfg with optimisations := rws) o' rws e0) e1’ \\ fs[]
+    \\ Cases_on ‘do_if (HD v) (perform_rewrites cfg o' rws e0) e1’ \\ fs[]
     \\ Cases_on ‘(HD v) = Boolv T’ \\ fs[do_if_def]
     \\ imp_res_tac evaluate_sing \\ fs[] \\ rveq
     (* HD v = Boolv T *)
     >- (
-      qpat_x_assum ‘∀ st1 st2 env cfg rws r path.
-                      _ ∧ _ ∧ _ ∧ _ ∧ evaluate _ _ [perform_rewrites _ _ _ e0] = _ ⇒ _’ drule
+      qpat_x_assum ‘! st1 st2 env cfg rws r path.
+                      _ /\ _ /\ _ /\ _ /\ evaluate _ _ [perform_rewrites _ _ _ e0] = _ ==> _’ drule
       \\ disch_then (qspecl_then [‘st'’, ‘st2’, ‘env’, ‘cfg’, ‘[v']’, ‘o'’] strip_assume_tac) \\ rfs[]
-      \\ ‘(st1.fp_state.canOpt = FPScope Opt ⇔
-           st'.fp_state.canOpt = FPScope Opt) ∧ st'.fp_state.canOpt ≠ Strict ∧
+      \\ ‘(st1.fp_state.canOpt = FPScope Opt <=>
+           st'.fp_state.canOpt = FPScope Opt) /\ st'.fp_state.canOpt <> Strict /\
           ~st'.fp_state.real_sem’ by (imp_res_tac evaluate_fp_opts_inv \\ fs[])
       \\ fs[]
       \\ fs[evaluate_def]
@@ -730,7 +730,7 @@ Proof
     qpat_x_assum ‘evaluate _ _ [If _ _ _] = _’ (
                    assume_tac o SIMP_RULE bool_ss [evaluate_def, CaseEq"prod", CaseEq"result"])
     \\ fs[] \\ rveq
-    \\ Cases_on ‘do_if (HD v) e0 (perform_rewrites (cfg with optimisations := rws) o' rws e1)’ \\ fs[]
+    \\ Cases_on ‘do_if (HD v) e0 (perform_rewrites cfg o' rws e1)’ \\ fs[]
     \\ Cases_on ‘(HD v) = Boolv T’ \\ fs[do_if_def]
     \\ imp_res_tac evaluate_sing \\ fs[] \\ rveq
     (* HD v = Boolv T *)
@@ -754,11 +754,11 @@ Proof
       )
     (* HD v = Boolv F *)
     >- (
-      qpat_x_assum ‘∀ st1 st2 env cfg rws r path.
-                      _ ∧ _ ∧ _ ∧ _ ∧ evaluate _ _ [perform_rewrites _ _ _ e1] = _ ⇒ _’ drule
+      qpat_x_assum ‘! st1 st2 env cfg rws r path.
+                      _ /\ _ /\ _ /\ _ /\ evaluate _ _ [perform_rewrites _ _ _ e1] = _ ==> _’ drule
       \\ disch_then (qspecl_then [‘st'’, ‘st2’, ‘env’, ‘cfg’, ‘[v']’, ‘o'’] strip_assume_tac) \\ rfs[]
-      \\ ‘(st1.fp_state.canOpt = FPScope Opt ⇔
-           st'.fp_state.canOpt = FPScope Opt) ∧ st'.fp_state.canOpt ≠ Strict ∧
+      \\ ‘(st1.fp_state.canOpt = FPScope Opt <=>
+           st'.fp_state.canOpt = FPScope Opt) /\ st'.fp_state.canOpt <> Strict /\
           ~st'.fp_state.real_sem’ by (imp_res_tac evaluate_fp_opts_inv \\ fs[])
       \\ fs[]
       \\ fs[evaluate_def]
@@ -781,8 +781,8 @@ Proof
     qpat_x_assum ‘evaluate _ _ [If _ _ _] = _’ (
                    assume_tac o SIMP_RULE bool_ss [evaluate_def, CaseEq"prod", CaseEq"result"])
     \\ fs[] \\ rveq
-    \\ qpat_x_assum ‘∀ st1 st2 env cfg rws r path.
-                       _ ∧ _ ∧ _ ∧ _ ∧ evaluate _ _ [perform_rewrites _ _ _ e] = _ ⇒ _’ drule
+    \\ qpat_x_assum ‘! st1 st2 env cfg rws r path.
+                       _ /\ _ /\ _ /\ _ /\ evaluate _ _ [perform_rewrites _ _ _ e] = _ ==> _’ drule
     \\ rpt (disch_then drule)
     \\ strip_tac
     \\ Cases_on ‘do_if (HD v) e0 e1’ \\ fs[]
@@ -815,15 +815,15 @@ Proof
     \\ fs[] \\ rveq
     \\ imp_res_tac evaluate_sing \\ rveq
     \\ fs[do_log_def]
-    \\ Cases_on ‘l = And ∧ v = Boolv T ∨ l = Or ∧ v = Boolv F’ \\ fs[]
+    \\ Cases_on ‘l = And /\ v = Boolv T \/ l = Or /\ v = Boolv F’ \\ fs[]
     \\ rveq \\ fs[]
-    (* l = And ∧ v = Boolv T and l = Or ∧ v = Boolv F *)
+    (* l = And /\ v = Boolv T and l = Or /\ v = Boolv F *)
     \\ TRY (
-      qpat_x_assum ‘∀ st1 st2 env cfg rws r path.
-                      _ ∧ _ ∧ _ ∧ _ ∧ evaluate _ _ [perform_rewrites _ _ _ e0] = _ ⇒ _’ drule
+      qpat_x_assum ‘! st1 st2 env cfg rws r path.
+                      _ /\ _ /\ _ /\ _ /\ evaluate _ _ [perform_rewrites _ _ _ e0] = _ ==> _’ drule
       \\ disch_then (qspecl_then [‘st'’, ‘st2’, ‘env’, ‘cfg’, ‘r’, ‘o'’] strip_assume_tac) \\ rfs[]
-      \\ ‘(st1.fp_state.canOpt = FPScope Opt ⇔
-           st'.fp_state.canOpt = FPScope Opt) ∧ st'.fp_state.canOpt ≠ Strict ∧
+      \\ ‘(st1.fp_state.canOpt = FPScope Opt <=>
+           st'.fp_state.canOpt = FPScope Opt) /\ st'.fp_state.canOpt <> Strict /\
           ~st'.fp_state.real_sem’ by (imp_res_tac evaluate_fp_opts_inv \\ fs[]) \\ fs[]
       \\ fs[evaluate_def]
       \\ qpat_x_assum ‘evaluate _ _ [e] = _’ (
@@ -853,7 +853,7 @@ Proof
       \\ fs[do_log_def]
       \\ fs[semState_comp_eq, fpState_component_equality]
       )
-    (* v ≠ Boolv T ∧ l ≠ Or *)
+    (* v <> Boolv T /\ l <> Or *)
     >- (
       Cases_on ‘l’ \\ fs[] \\ Cases_on ‘v = Boolv F’ \\ fs[] \\ rveq \\ fs[]
       \\ fs[evaluate_def]
@@ -873,8 +873,8 @@ Proof
     qpat_x_assum ‘evaluate _ _ [Log _ _ _] = _’ (
                    assume_tac o SIMP_RULE bool_ss [evaluate_def, CaseEq"prod", CaseEq"result"])
     \\ fs[] \\ rveq
-    \\ qpat_x_assum ‘∀ st1 st2 env cfg rws r path.
-                       _ ∧ _ ∧ _ ∧ _ ∧ evaluate _ _ [perform_rewrites _ _ _ e] = _ ⇒ _’ drule
+    \\ qpat_x_assum ‘! st1 st2 env cfg rws r path.
+                       _ /\ _ /\ _ /\ _ /\ evaluate _ _ [perform_rewrites _ _ _ e] = _ ==> _’ drule
     \\ rpt (disch_then drule)
     \\ strip_tac
     \\ Cases_on ‘do_log l (HD v1) e0’ \\ fs[]
@@ -913,14 +913,14 @@ Proof
     qpat_x_assum ‘evaluate _ _ [Let _ _ _] = _’ (
                    assume_tac o SIMP_RULE bool_ss [evaluate_def, CaseEq"prod", CaseEq"result"])
     \\ fs[] \\ rveq
-    \\ qpat_x_assum ‘∀ st1 st2 env cfg rws r path.
-                       _ ∧ _ ∧ _ ∧ _ ∧ evaluate _ _ [perform_rewrites _ _ _ e0] = _ ⇒ _’ drule
+    \\ qpat_x_assum ‘! st1 st2 env cfg rws r path.
+                       _ /\ _ /\ _ /\ _ /\ evaluate _ _ [perform_rewrites _ _ _ e0] = _ ==> _’ drule
     \\ disch_then (
       qspecl_then [
           ‘st'’, ‘st2’, ‘(env with v := nsOptBind o' (HD v) env.v)’, ‘cfg’, ‘r’, ‘o''’
         ] strip_assume_tac) \\ rfs[]
-    \\ ‘(st1.fp_state.canOpt = FPScope Opt ⇔
-           st'.fp_state.canOpt = FPScope Opt) ∧ st'.fp_state.canOpt ≠ Strict ∧
+    \\ ‘(st1.fp_state.canOpt = FPScope Opt <=>
+           st'.fp_state.canOpt = FPScope Opt) /\ st'.fp_state.canOpt <> Strict /\
           ~st'.fp_state.real_sem’ by (imp_res_tac evaluate_fp_opts_inv \\ fs[]) \\ fs[]
     \\ qpat_x_assum ‘evaluate _ _ [e] = _’ (
                       mp_then Any assume_tac (prep (CONJUNCT1 evaluate_fp_rws_append)))
@@ -939,8 +939,8 @@ Proof
     qpat_x_assum ‘evaluate _ _ [Let _ _ _] = _’ (
                    assume_tac o SIMP_RULE bool_ss [evaluate_def, CaseEq"prod", CaseEq"result"])
     \\ fs[] \\ rveq
-    \\ qpat_x_assum ‘∀ st1 st2 env cfg rws r path.
-                       _ ∧ _ ∧ _ ∧ _ ∧ evaluate _ _ [perform_rewrites _ _ _ e] = _ ⇒ _’ drule
+    \\ qpat_x_assum ‘! st1 st2 env cfg rws r path.
+                       _ /\ _ /\ _ /\ _ /\ evaluate _ _ [perform_rewrites _ _ _ e] = _ ==> _’ drule
     \\ rpt (disch_then drule)
     \\ strip_tac
     \\ fs[evaluate_def]
@@ -958,15 +958,15 @@ Proof
   (* Case: ?? *)
   >- (
   rveq
-  \\ qpat_x_assum ‘∀ st1 st2 env cfg rws r path.
-                     _ ∧ _ ∧ _ ∧ _ ∧ evaluate _ _ [perform_rewrites _ _ _ e] = _ ⇒ _’ drule
+  \\ qpat_x_assum ‘! st1 st2 env cfg rws r path.
+                     _ /\ _ /\ _ /\ _ /\ evaluate _ _ [perform_rewrites _ _ _ e] = _ ==> _’ drule
   \\ rpt (disch_then drule)
   \\ fs[])
   (* Case: ?? *)
   >- (
   rveq
-  \\ qpat_x_assum ‘∀ e. MEM e l ⇒ ∀ st1 st2 env cfg rws r path.
-                                    _ ∧ _ ∧ _ ∧ _ ∧ evaluate _ _ [perform_rewrites _ _ _ _] = _ ⇒ _’ drule
+  \\ qpat_x_assum ‘! e. MEM e l ==> ! st1 st2 env cfg rws r path.
+                                    _ /\ _ /\ _ /\ _ /\ evaluate _ _ [perform_rewrites _ _ _ _] = _ ==> _’ drule
   \\ rpt (disch_then drule)
   \\ fs[])
   (* Case: Handle e l *)
@@ -987,18 +987,18 @@ Proof
     \\ fs[] \\ rveq
     \\ Cases_on ‘can_pmatch_all env.c st'.refs
                  (MAPi
-                  ($o FST ∘
+                  ($o FST o
                    (λn (p,e').
                     if n = q then
-                      (p, perform_rewrites (cfg with optimisations := rws) r' rws e')
+                      (p, perform_rewrites cfg r' rws e')
                     else (p,e'))) l) (HD v)’ \\ fs[]
-    \\ qpat_x_assum ‘∀ st1 st2 env cfg rws r v err_v path i.
-                       _ ∧ _ ∧ _ ∧ _ ∧ evaluate_match _ _ _ _ _ = _ ⇒ _’ drule
+    \\ qpat_x_assum ‘! st1 st2 env cfg rws r v err_v path i.
+                       _ /\ _ /\ _ /\ _ /\ evaluate_match _ _ _ _ _ = _ ==> _’ drule
     \\ disch_then (qspecl_then [
                       ‘st'’, ‘st2’, ‘env’, ‘cfg’, ‘r’, ‘HD v’, ‘bind_exn_v’, ‘r'’, ‘q’ ] strip_assume_tac)
     \\ rfs[]
-    \\ ‘(st1.fp_state.canOpt = FPScope Opt ⇔
-         st'.fp_state.canOpt = FPScope Opt) ∧ st'.fp_state.canOpt ≠ Strict ∧
+    \\ ‘(st1.fp_state.canOpt = FPScope Opt <=>
+         st'.fp_state.canOpt = FPScope Opt) /\ st'.fp_state.canOpt <> Strict /\
         ~st'.fp_state.real_sem’ by (imp_res_tac evaluate_fp_opts_inv \\ fs[]) \\ fs[]
     \\ fs[evaluate_def]
     \\ qpat_x_assum ‘evaluate _ _ [e] = _’ (
@@ -1007,24 +1007,24 @@ Proof
     \\ qpat_x_assum ‘evaluate _ _ [e] = _’ (mp_then Any mp_tac (CONJUNCT1 evaluate_add_choices))
     \\ disch_then (qspec_then ‘st1.fp_state.choices’ assume_tac) \\ fs[]
     \\ qexistsl_tac [‘fpOpt'’, ‘st1.fp_state.choices’] \\ fs[]
-    \\ ‘($o FST ∘
+    \\ ‘($o FST o
          (λn (p,e').
           if n = q then
-            (p, perform_rewrites (cfg with optimisations := rws) r' rws e')
+            (p, perform_rewrites cfg r' rws e')
           else (p,e'))) = (λ n (p, e'). p)’ by (
       fs[FUN_EQ_THM]
       \\ rpt strip_tac \\ Cases_on ‘x’ \\ fs[] \\ Cases_on ‘n = q’ \\ fs[]
       )
-    \\ ‘(MAPi ($o FST ∘
+    \\ ‘(MAPi ($o FST o
                (λn (p,e').
                 if n = q then
-                  (p, perform_rewrites (cfg with optimisations := rws) r' rws e')
+                  (p, perform_rewrites cfg r' rws e')
                 else (p,e'))) l) =
         (MAPi (λ n (p, e'). p) l)’ by (
-      qspecl_then [‘l’, ‘l’, ‘($o FST ∘
+      qspecl_then [‘l’, ‘l’, ‘($o FST o
                                (λn (p,e').
                                 if n = q then
-                                  (p, perform_rewrites (cfg with optimisations := rws) r' rws e')
+                                  (p, perform_rewrites cfg r' rws e')
                                 else (p,e')))’, ‘(λ n (p, e'). p)’] strip_assume_tac MAPi_CONG
       \\ imp_res_tac FUN_EQ_THM
       \\ fs[]
@@ -1032,7 +1032,7 @@ Proof
       \\ fs[FUN_EQ_THM, FORALL_PROD] \\ rw[]
       )
     \\ fs[]
-    \\ ‘∀ l: (pat # exp) list. MAPi (λ n (p, e'). p) l = MAP FST l’ by (
+    \\ ‘! l: (pat # exp) list. MAPi (λ n (p, e'). p) l = MAP FST l’ by (
       Induct \\ fs[]
       \\ fs[FORALL_PROD, o_DEF]
       )
@@ -1061,8 +1061,8 @@ Proof
     qpat_x_assum ‘evaluate _ _ [Mat _ _] = _’ (
                    assume_tac o SIMP_RULE bool_ss [evaluate_def, CaseEq"prod", CaseEq"result"])
     \\ fs[] \\ rveq
-    \\ qpat_x_assum ‘∀ st1 st2 env cfg rws r path.
-                       _ ∧ _ ∧ _ ∧ _ ∧ evaluate _ _ [perform_rewrites _ _ _ e] = _ ⇒ _’ drule
+    \\ qpat_x_assum ‘! st1 st2 env cfg rws r path.
+                       _ /\ _ /\ _ /\ _ /\ evaluate _ _ [perform_rewrites _ _ _ e] = _ ==> _’ drule
     \\ rpt (disch_then drule)
     \\ strip_tac
     \\ fs[evaluate_def]
@@ -1071,7 +1071,7 @@ Proof
                       mp_then Any assume_tac (prep (CONJUNCT2 evaluate_fp_rws_append)))
     \\ first_x_assum (qspecl_then [‘rws’, ‘st2.fp_state.opts’] assume_tac) \\ fs[]
     \\ optUntil_tac ‘evaluate _ _ [e] = _’ ‘fpOpt'’
-    \\ qexistsl_tac [‘optUntil (choicesR − choices) fpOpt fpOpt'’, ‘choices’] \\ fs[]
+    \\ qexistsl_tac [‘optUntil (choicesR - choices) fpOpt fpOpt'’, ‘choices’] \\ fs[]
     \\ Cases_on ‘l’ \\ fs[evaluate_def] \\ Cases_on ‘h’ \\ fs[evaluate_def]
     \\ Cases_on ‘ALL_DISTINCT (pat_bindings q [])’ \\ fs[]
     \\ Cases_on ‘pmatch env.c st'.refs q (HD v) []’ \\ fs[]
@@ -1096,8 +1096,8 @@ Proof
     qpat_x_assum ‘evaluate _ _ [Tannot _ _] = _’ (
                    assume_tac o SIMP_RULE bool_ss [evaluate_def, CaseEq"prod", CaseEq"result"])
     \\ fs[] \\ rveq
-    \\ qpat_x_assum ‘∀ st1 st2 env cfg rws r path.
-                       _ ∧ _ ∧ _ ∧ _ ∧ evaluate _ _ [perform_rewrites _ _ _ e] = _ ⇒ _’ drule
+    \\ qpat_x_assum ‘! st1 st2 env cfg rws r path.
+                       _ /\ _ /\ _ /\ _ /\ evaluate _ _ [perform_rewrites _ _ _ e] = _ ==> _’ drule
     \\ rpt (disch_then drule)
     \\ strip_tac
     \\ fs[evaluate_def]
@@ -1121,13 +1121,13 @@ Proof
                  (st1 with fp_state :=
                   if st1.fp_state.canOpt = Strict then st1.fp_state
                   else st1.fp_state with canOpt := FPScope f) env
-                 [perform_rewrites <|optimisations := rws; canOpt := (f = Opt)|> o' rws e]’ \\ fs[]
+                 [perform_rewrites (cfg with canOpt := (f = Opt)) o' rws e]’ \\ fs[]
     \\ Cases_on ‘r'’ \\ fs[] \\ rveq \\ fs[]
     \\ Cases_on ‘st1.fp_state.canOpt = Strict’ \\ fs[]
-    \\ qpat_x_assum ‘∀ st1 st2 env cfg rws r path.
-                       _ ∧ _ ∧ _ ∧ _ ∧ evaluate _ _ [perform_rewrites _ _ _ e] = _ ⇒ _’ drule
+    \\ qpat_x_assum ‘! st1 st2 env cfg rws r path.
+                       _ /\ _ /\ _ /\ _ /\ evaluate _ _ [perform_rewrites _ _ _ e] = _ ==> _’ drule
     \\ disch_then (qspecl_then [‘st1 with fp_state := st1.fp_state with canOpt := FPScope f’,
-                               ‘q’, ‘env’, ‘<|optimisations := rws; canOpt := (f = Opt)|>’,
+                               ‘q’, ‘env’, ‘cfg with canOpt := (f = Opt)’,
                                ‘a’, ‘o'’] strip_assume_tac)
     \\ rfs[]
     \\ fs[evaluate_def]
@@ -1138,8 +1138,8 @@ Proof
   )
   (* Case: ?? *)
   >- (
-  qpat_x_assum ‘∀ st1 st2 env cfg rws r path.
-                  _ ∧ _ ∧ _ ∧ _ ∧ evaluate _ _ [perform_rewrites _ _ _ e] = _ ⇒ _’ drule
+  qpat_x_assum ‘! st1 st2 env cfg rws r path.
+                  _ /\ _ /\ _ /\ _ /\ evaluate _ _ [perform_rewrites _ _ _ e] = _ ==> _’ drule
   \\ rpt (disch_then drule)
   \\ fs[])
   (* Case: Fun s e *)
@@ -1158,8 +1158,8 @@ Proof
     qpat_x_assum ‘evaluate _ _ [Lannot _ _] = _’ (
                    assume_tac o SIMP_RULE bool_ss [evaluate_def, CaseEq"prod", CaseEq"result"])
     \\ fs[] \\ rveq
-    \\ qpat_x_assum ‘∀ st1 st2 env cfg rws r path.
-                       _ ∧ _ ∧ _ ∧ _ ∧ evaluate _ _ [perform_rewrites _ _ _ e] = _ ⇒ _’ drule
+    \\ qpat_x_assum ‘! st1 st2 env cfg rws r path.
+                       _ /\ _ /\ _ /\ _ /\ evaluate _ _ [perform_rewrites _ _ _ e] = _ ==> _’ drule
     \\ rpt (disch_then drule)
     \\ strip_tac
     \\ fs[evaluate_def]
@@ -1168,8 +1168,8 @@ Proof
   \\ no_change_tac ‘Lannot e a’)
   (* Case: ?? *)
   >- (
-  qpat_x_assum ‘∀ st1 st2 env cfg rws r path.
-                  _ ∧ _ ∧ _ ∧ _ ∧ evaluate _ _ [perform_rewrites _ _ _ e] = _ ⇒ _’ drule
+  qpat_x_assum ‘! st1 st2 env cfg rws r path.
+                  _ /\ _ /\ _ /\ _ /\ evaluate _ _ [perform_rewrites _ _ _ e] = _ ==> _’ drule
   \\ rpt (disch_then drule)
   \\ fs[])
   (* Case: Raise e *)
@@ -1219,11 +1219,11 @@ Proof
     \\ fs[] \\ rveq
     \\ qspecl_then [‘(λ(n, e).
                         if n = q then
-                          perform_rewrites (cfg with optimisations := rws) r' rws e
+                          perform_rewrites cfg r' rws e
                         else e)’, ‘l’] strip_assume_tac MAP_enumerate_MAPi
     \\ fs[EVAL “(λn e. (λ(n,e).
                           if n = q then
-                            perform_rewrites (cfg with optimisations := rws) r' rws e
+                            perform_rewrites cfg r' rws e
                           else e) (n,e))”]
     \\ pop_assum (assume_tac o GSYM) \\ fs[]
     \\ pop_assum kall_tac
@@ -1244,7 +1244,7 @@ Proof
                       mp_then Any assume_tac (prep (CONJUNCT1 evaluate_fp_rws_append)))
       \\ pop_assum (qspecl_then [‘rws’, ‘st2.fp_state.opts’] strip_assume_tac)
       \\ optUntil_tac ‘evaluate _ _ (REVERSE l) = _’ ‘fpOpt'’
-      \\ qexistsl_tac [‘optUntil (choicesR − choices) fpOpt fpOpt'’, ‘choices’] \\ fs[]
+      \\ qexistsl_tac [‘optUntil (choicesR - choices) fpOpt fpOpt'’, ‘choices’] \\ fs[]
       \\ fs[dec_clock_def, semState_comp_eq, fpState_component_equality]
       \\ qpat_x_assum ‘evaluate _ _ [r''] = _’ (mp_then Any mp_tac (CONJUNCT1 evaluate_add_choices))
       \\ fs[semState_comp_eq, fpState_component_equality]
@@ -1268,7 +1268,7 @@ Proof
          \\ imp_res_tac do_fprw_append_opt
          \\ first_x_assum (qspec_then ‘rws’ strip_assume_tac)
          \\ optUntil_tac ‘evaluate _ _ (REVERSE l) = _’ ‘λ x. if (x = 0) then sched2 else st1N.fp_state.opts x’
-         \\ qexistsl_tac [‘optUntil (choicesR − choices) fpOpt
+         \\ qexistsl_tac [‘optUntil (choicesR - choices) fpOpt
                            (λx. if x = 0 then sched2 else st1N.fp_state.opts x)’, ‘choices’] \\ fs[]
          \\ fsrw_tac [SATISFY_ss] [shift_fp_opts_def, semState_comp_eq, fpState_component_equality]
         )
@@ -1299,11 +1299,11 @@ Proof
     \\ Cases_on ‘do_con_check env.c o' (LENGTH l)’ \\ fs[]
     \\ qspecl_then [‘(λ(n, e).
                         if n = q then
-                          perform_rewrites (cfg with optimisations := rws) r' rws e
+                          perform_rewrites cfg r' rws e
                         else e)’, ‘l’] strip_assume_tac MAP_enumerate_MAPi
     \\ fs[EVAL “(λn e. (λ(n,e).
                           if n = q then
-                            perform_rewrites (cfg with optimisations := rws) r' rws e
+                            perform_rewrites cfg r' rws e
                           else e) (n,e))”]
     \\ pop_assum (assume_tac o GSYM) \\ fs[]
     \\ pop_assum kall_tac
@@ -1315,7 +1315,7 @@ Proof
                  (MAP
                   (λ(n,e).
                      if n = q then
-                       perform_rewrites (cfg with optimisations := rws) r'
+                       perform_rewrites cfg r'
                                         rws e
                      else e) (REVERSE (enumerate 0 l)))’ \\ fs[]
     \\ Cases_on ‘r''’ \\ fs[] \\ Cases_on ‘build_conv env.c o' (REVERSE a)’ \\ fs[] \\ rveq
@@ -1341,8 +1341,8 @@ Proof
     \\ fs[] \\ rveq
     \\ Cases_on ‘ALL_DISTINCT (MAP (λ(x,y,z). x) l)’ \\ fs[]
     \\ fs[evaluate_def]
-    \\ qpat_x_assum ‘∀ st1 st2 env cfg rws r path.
-                       _ ∧ _ ∧ _ ∧ _ ∧ evaluate _ _ [perform_rewrites _ _ _ e] = _ ⇒ _’ mp_tac
+    \\ qpat_x_assum ‘! st1 st2 env cfg rws r path.
+                       _ /\ _ /\ _ /\ _ /\ evaluate _ _ [perform_rewrites _ _ _ e] = _ ==> _’ mp_tac
     \\ disch_then (qspecl_then [‘st1’, ‘st2’, ‘(env with v := build_rec_env l env env.v)’,
                                 ‘cfg’, ‘rws’, ‘r’, ‘o'’] strip_assume_tac)
     \\ rfs[]
@@ -1373,7 +1373,7 @@ Proof
   Cases_on ‘p’ \\ Cases_on ‘i = 0’ \\ fs[]
   \\ fs[o_DEF]
   >- (
-    ‘∀l: (pat # exp) list. MAPi (λ x (n, e'). (n, e')) l = l’ by (
+    ‘!l: (pat # exp) list. MAPi (λ x (n, e'). (n, e')) l = l’ by (
       Induct \\ fs[]
       \\ fs[FORALL_PROD, o_DEF]
       )
@@ -1390,8 +1390,8 @@ Proof
       \\ fs[semState_comp_eq, fpState_component_equality]
       )
     >- (
-      qpat_x_assum ‘∀ st1 st2 env cfg rws r path.
-                       _ ∧ _ ∧ _ ∧ _ ∧ evaluate _ _ [perform_rewrites _ _ _ r'] = _ ⇒ _’ mp_tac
+      qpat_x_assum ‘! st1 st2 env cfg rws r path.
+                       _ /\ _ /\ _ /\ _ /\ evaluate _ _ [perform_rewrites _ _ _ r'] = _ ==> _’ mp_tac
       \\ disch_then (qspecl_then [‘st1’, ‘st2’, ‘(env with v := nsAppend (alist_to_ns a) env.v)’,
                                   ‘cfg’, ‘rws’, ‘r’, ‘path’] strip_assume_tac)
       \\ rfs[]
@@ -1407,15 +1407,15 @@ Proof
       \\ qmatch_goalsub_abbrev_tac ‘evaluate_match _ _ _ (MAPi selFun _) _ = _’
       \\ ‘selFun = λx (p,e).
                     if x = i - 1 then
-                      (p, perform_rewrites (cfg with optimisations := rws) path rws e)
+                      (p, perform_rewrites cfg path rws e)
                     else (p,e)’ by (
         unabbrev_all_tac \\ fs[FUN_EQ_THM]
         \\ rpt strip_tac \\ TOP_CASE_TAC \\ fs[]
         )
       \\ pop_assum (rewrite_tac o single)
       \\ rpt strip_tac \\ unabbrev_all_tac
-      \\ qpat_x_assum ‘∀st1 st2 env cfg rws r v err_v path i.
-                      _ ∧ _ ∧ _ ∧ _ ∧ evaluate_match _ _ _ _ _ = _ ⇒ _’ (
+      \\ qpat_x_assum ‘!st1 st2 env cfg rws r v err_v path i.
+                      _ /\ _ /\ _ /\ _ /\ evaluate_match _ _ _ _ _ = _ ==> _’ (
                         qspecl_then [
                             ‘st1’, ‘st2’, ‘env’, ‘cfg’, ‘rws’, ‘r’, ‘v’, ‘err_v’, ‘path’, ‘i - 1’
                           ] strip_assume_tac
@@ -1440,11 +1440,11 @@ Proof
 QED
 
 Theorem is_rewriteFPexp_correct_lift_perform_rewrites:
-  ∀ rws.
-    (∀ (st1 st2:'a semanticPrimitives$state) env e r.
-       is_rewriteFPexp_list_correct rws st1 st2 env e r) ⇒
-    (∀ path (st1 st2:'a semanticPrimitives$state) env cfg e r.
-       is_perform_rewrites_correct rws st1 st2 env (cfg with optimisations := rws) e r path)
+  ! rws.
+    (! (st1 st2:'a semanticPrimitives$state) env e r.
+       is_rewriteFPexp_list_correct rws st1 st2 env e r) ==>
+    (! path (st1 st2:'a semanticPrimitives$state) env cfg e r.
+       is_perform_rewrites_correct rws st1 st2 env cfg e r path)
 Proof
   rpt strip_tac
   \\ simp[is_perform_rewrites_correct_def]
@@ -1469,12 +1469,12 @@ Proof
 QED
 
 Theorem is_optimise_with_plan_correct_lift_sing:
-  ∀ plan.
-    (∀ rws path.
-       MEM (Apply (path, rws)) plan ⇒
-       ∀ (st1:'a semanticPrimitives$state) st2 env cfg e r.
-         is_perform_rewrites_correct rws st1 st2 env (cfg with optimisations := rws) e r path) ⇒
-    (∀ (st1:'a semanticPrimitives$state) st2 env cfg e r.
+  ! plan.
+    (! rws path.
+       MEM (Apply (path, rws)) plan ==>
+       ! (st1:'a semanticPrimitives$state) st2 env cfg e r.
+         is_perform_rewrites_correct rws st1 st2 env cfg e r path) ==>
+    (! (st1:'a semanticPrimitives$state) st2 env cfg e r.
        is_optimise_with_plan_correct plan st1 st2 env cfg [e] r)
 Proof
   Induct_on ‘plan’
@@ -1535,7 +1535,7 @@ Proof
     rpt strip_tac \\ rfs[is_perform_rewrites_correct_def] \\ rveq
     \\ qpat_assum `evaluate _ _ _ = _` (fn th => first_x_assum (fn thm => mp_then Any assume_tac thm th))
     \\ rfs[] \\ asm_exists_tac \\ fs[])
-  \\ Cases_on ‘optimise_with_plan cfg plan (perform_rewrites (cfg with optimisations := r') q r' e)’
+  \\ Cases_on ‘optimise_with_plan cfg plan (perform_rewrites cfg q r' e)’
   \\ fs[]
   \\ COND_CASES_TAC \\ fs[] \\ rveq
   >- (
@@ -1552,7 +1552,7 @@ Proof
   \\ rpt strip_tac
   \\ first_x_assum (qspecl_then [‘r'’, ‘q’] mp_tac) \\ fs[] \\ strip_tac
   \\ fs[is_optimise_with_plan_correct_def]
-  \\ last_x_assum (qspecl_then [‘st1’, ‘st2’, ‘env’, ‘cfg’, ‘perform_rewrites (cfg with optimisations := r') q r' e’, ‘r’] mp_tac)
+  \\ last_x_assum (qspecl_then [‘st1’, ‘st2’, ‘env’, ‘cfg’, ‘perform_rewrites cfg q r' e’, ‘r’] mp_tac)
   \\ impl_tac \\ fs[]
   \\ strip_tac
   \\ fs[is_perform_rewrites_correct_def]
@@ -1586,12 +1586,12 @@ Proof
 QED
 
 Theorem is_optimise_with_plan_correct_lift:
-  ∀ plan.
-    (∀ rws path.
-       MEM (Apply (path, rws)) plan ⇒
-       ∀ (st1:'a semanticPrimitives$state) st2 env cfg e r.
-         is_perform_rewrites_correct rws st1 st2 env (cfg with optimisations := rws) e r path) ⇒
-    (∀ (st1:'a semanticPrimitives$state) st2 env cfg exps r.
+  ! plan.
+    (! rws path.
+       MEM (Apply (path, rws)) plan ==>
+       ! (st1:'a semanticPrimitives$state) st2 env cfg e r.
+         is_perform_rewrites_correct rws st1 st2 env cfg e r path) ==>
+    (! (st1:'a semanticPrimitives$state) st2 env cfg exps r.
        is_optimise_with_plan_correct plan st1 st2 env cfg exps r)
 Proof
   ntac 2 strip_tac
@@ -1608,18 +1608,18 @@ Proof
   \\ first_x_assum (qspecl_then [‘s'’, ‘s''’, ‘env’, ‘cfg’, ‘vs'’] strip_assume_tac)
   \\ fs[is_optimise_with_plan_correct_def]
   \\ rfs[] \\ fs[]
-  \\ ‘(st1.fp_state.canOpt = FPScope Opt ⇔ s'.fp_state.canOpt = FPScope Opt) ∧
-        s'.fp_state.canOpt ≠ Strict ∧ ~s'.fp_state.real_sem’ by (imp_res_tac evaluate_fp_opts_inv \\ fs[])
+  \\ ‘(st1.fp_state.canOpt = FPScope Opt <=> s'.fp_state.canOpt = FPScope Opt) /\
+        s'.fp_state.canOpt <> Strict /\ ~s'.fp_state.real_sem’ by (imp_res_tac evaluate_fp_opts_inv \\ fs[])
   \\ fs[]
   \\ optUntil_tac ‘evaluate _ _ [h] = _’ ‘fpOpt'’
-  \\ qexistsl_tac [‘optUntil (choicesR − choices) fpOpt fpOpt'’, ‘choices’] \\ fs[]
+  \\ qexistsl_tac [‘optUntil (choicesR - choices) fpOpt fpOpt'’, ‘choices’] \\ fs[]
   \\ qpat_x_assum ‘evaluate _ _ exps = _’ (mp_then Any mp_tac (CONJUNCT1 evaluate_add_choices))
   \\ disch_then (qspec_then ‘choicesR’ assume_tac)
   \\ fs[semState_comp_eq, fpState_component_equality]
 QED
 
 Theorem stos_pass_with_plans_sing_exists:
-  ∀ e plan. ∃ e_opt res. HD (stos_pass_with_plans cfg [plan] [e]) = (e_opt, res)
+  ! e plan. ? e_opt res. HD (stos_pass_with_plans cfg [plan] [e]) = (e_opt, res)
 Proof
   rpt strip_tac \\ measureInduct_on ‘exp_size e’ \\ Cases_on ‘e’
   \\ simp[stos_pass_with_plans_def]
@@ -1646,7 +1646,7 @@ Proof
 QED
 
 Theorem stos_pass_with_plans_empty:
-  ∀ e. stos_pass_with_plans cfg [] [e] = [(e, Success)]
+  ! e. stos_pass_with_plans cfg [] [e] = [(e, Success)]
 Proof
   strip_tac \\ measureInduct_on ‘exp_size e’ \\ Cases_on ‘e’
   \\ fs[stos_pass_with_plans_def]
@@ -1655,8 +1655,7 @@ Proof
 QED
 
 Theorem stos_pass_with_plans_cons:
-  ∀ plan1 plans e1 es cfg.
-  LENGTH es <= LENGTH plans ⇒
+  ! plan1 plans e1 es cfg.
   stos_pass_with_plans cfg (plan1::plans) (e1::es) =
   stos_pass_with_plans cfg [plan1] [e1] ++ stos_pass_with_plans cfg plans es
 Proof
@@ -1682,10 +1681,7 @@ Proof
           Once stos_pass_with_plans_decs_cons, no_optimise_pass_def, HD,
           stos_pass_with_plans_def, stos_pass_with_plans_empty]
   \\ qspecl_then [‘e’, ‘h’] strip_assume_tac stos_pass_with_plans_sing_exists
-  \\ fs[]
-  \\ qspecl_then [‘h’, ‘t’, ‘e’, ‘[]’, ‘cfg’] mp_tac stos_pass_with_plans_cons
-  \\ impl_tac \\ fs[]
-  \\ strip_tac \\ fs[stos_pass_with_plans_def]
+  \\ fs[Once stos_pass_with_plans_cons, stos_pass_with_plans_def]
   \\ simp[no_opt_decs_def]
 QED
 
@@ -1697,16 +1693,16 @@ Proof
   \\ simp[stos_pass_with_plans_def, no_optimise_pass_def,Once  optimise_with_plan_def,
           Once stos_pass_with_plans_cons,
           stos_pass_with_plans_sing, stos_pass_with_plans_empty]
-  \\ qspecl_then [‘h’, ‘t’, ‘e’, ‘[]’, ‘cfg’] mp_tac stos_pass_with_plans_cons
-  \\ impl_tac \\ fs[]
-  \\ strip_tac \\ fs[stos_pass_with_plans_def]
+  \\ qspecl_then [‘h’, ‘t’,‘e’, ‘[]’, ‘cfg’] assume_tac stos_pass_with_plans_cons
+  \\ pop_assum (rewrite_tac o single)
+  \\ fs[stos_pass_with_plans_def]
   \\ qspecl_then [‘e’, ‘h’] strip_assume_tac stos_pass_with_plans_sing_exists
   \\ fs[no_optimise_pass_def]
 QED
 
 Theorem optimise_with_plan_scope:
-  ∀ cfg plan sc e x. optimise_with_plan cfg plan (FpOptimise sc e) = x ⇒
-  ∃e' res. x = (FpOptimise sc e', res)
+  ! cfg plan sc e x. optimise_with_plan cfg plan (FpOptimise sc e) = x ==>
+  ?e' res. x = (FpOptimise sc e', res)
 Proof
   Induct_on ‘plan’
   >- fs[optimise_with_plan_empty_sing]
@@ -1720,7 +1716,7 @@ Proof
       \\ COND_CASES_TAC \\ strip_tac \\ rveq \\ fsrw_tac [SATISFY_ss] []
       \\ COND_CASES_TAC \\ rveq \\ TRY (Cases_on ‘q’
                                         \\ fsrw_tac [SATISFY_ss] [perform_rewrites_def])
-      \\ first_x_assum $ qspecl_then [‘cfg’, ‘sc’, ‘perform_rewrites <|optimisations := r; canOpt := (sc = Opt)|> o' r e’] strip_assume_tac
+      \\ first_x_assum $ qspecl_then [‘cfg’, ‘sc’, ‘perform_rewrites (cfg with canOpt := (sc = Opt)) o' r e’] strip_assume_tac
       \\ fs[]
       \\ COND_CASES_TAC \\ rveq \\ fsrw_tac [SATISFY_ss] [])
     \\ fs[optimise_with_plan_def] \\ metis_tac[])
@@ -1740,27 +1736,27 @@ Proof
 QED
 
 Theorem genlist_is_all_distinct:
-  ∀ f i. (∀ a b. a ≠ b ⇒ f a ≠ f b) ⇒ ALL_DISTINCT (GENLIST f i)
+  ! f i. (! a b. a <> b ==> f a <> f b) ==> ALL_DISTINCT (GENLIST f i)
 Proof
   fs[ALL_DISTINCT_GENLIST]
   \\ rpt strip_tac
-  \\ qpat_x_assum ‘∀ a b. _ ⇒ _’ (qspecl_then [‘m1’, ‘m2’] strip_assume_tac)
-  \\ qspecl_then [‘m1 ≠ m2’, ‘f m1 ≠ f m2’] strip_assume_tac (GEN_ALL MONO_NOT_EQ) \\ fs[]
+  \\ qpat_x_assum ‘! a b. _ ==> _’ (qspecl_then [‘m1’, ‘m2’] strip_assume_tac)
+  \\ qspecl_then [‘m1 <> m2’, ‘f m1 <> f m2’] strip_assume_tac (GEN_ALL MONO_NOT_EQ) \\ fs[]
 QED
 
 Theorem FIND_exists:
-  ∀ P l. (∃ x. MEM x l ∧ P x) ⇒ FIND P l ≠ NONE
+  ! P l. (? x. MEM x l /\ P x) ==> FIND P l <> NONE
 Proof
   Induct_on ‘l’ \\ fs[]
   \\ rpt strip_tac
-  \\ qpat_x_assum ‘∀P. _ ⇒ _’ (qspec_then ‘P’ assume_tac)
+  \\ qpat_x_assum ‘!P. _ ==> _’ (qspec_then ‘P’ assume_tac)
   \\ fs[FIND_thm] \\ rveq
   \\ Cases_on ‘P h’ \\ fs[]
-  \\ qpat_x_assum ‘_ ⇒ _’ imp_res_tac
+  \\ qpat_x_assum ‘_ ==> _’ imp_res_tac
 QED
 
 Theorem longer_and_distinct_exists:
-  ∀ l l'. ALL_DISTINCT l ∧ LENGTH l > LENGTH l' ⇒ ∃ x. MEM x l ∧ ~ MEM x l'
+  ! l l'. ALL_DISTINCT l /\ LENGTH l > LENGTH l' ==> ? x. MEM x l /\ ~ MEM x l'
 Proof
   rpt strip_tac
   \\ qspec_then ‘set l'’ strip_assume_tac LESS_CARD_DIFF \\ fs[]
@@ -1770,14 +1766,14 @@ Proof
   \\ fs[]
   \\ ‘CARD (set l') < LENGTH l’ by fs[]
   \\ fs[]
-  \\ ‘CARD (set l) − CARD (set l ∩ set l') = CARD ((set l) DIFF (set l'))’ by fs[CARD_DIFF_EQN]
+  \\ ‘CARD (set l) - CARD (set l INTER set l') = CARD ((set l) DIFF (set l'))’ by fs[CARD_DIFF_EQN]
   \\ ‘0 < CARD (set l DIFF set l')’ by fs[]
-  \\ ‘(set l DIFF set l') ≠ ∅’ by (
+  \\ ‘(set l DIFF set l') <> {} ’ by (
     qspec_then ‘set l DIFF set l'’ strip_assume_tac CARD_EQ_0
     \\ ‘FINITE (set l DIFF set l')’ by fs[FINITE_DIFF]
-    \\ qpat_x_assum ‘FINITE _ ⇒ _’ imp_res_tac
-    \\ Cases_on ‘set l DIFF set l' = ∅’ \\ simp[]
-    \\ qpat_x_assum ‘set l DIFF set l' = ∅ ⇒ CARD (set l DIFF set l') = 0’ imp_res_tac
+    \\ qpat_x_assum ‘FINITE _ ==> _’ imp_res_tac
+    \\ Cases_on ‘set l DIFF set l' = {} ’ \\ simp[]
+    \\ qpat_x_assum ‘set l DIFF set l' = {} ==> CARD (set l DIFF set l') = 0’ imp_res_tac
     \\ pop_assum mp_tac \\ qpat_x_assum ‘0 < CARD (set l DIFF set l')’ mp_tac
     \\ rpt (pop_assum kall_tac)
     \\ rpt strip_tac
@@ -1791,17 +1787,17 @@ Proof
 QED
 
 Theorem all_distinct_MEM_FIND:
-  ∀ l l'. ALL_DISTINCT l ∧ LENGTH l > LENGTH l' ⇒ FIND (λ x. ~MEM x l') l = v ⇒ v ≠ NONE
+  ! l l'. ALL_DISTINCT l /\ LENGTH l > LENGTH l' ==> FIND (λ x. ~MEM x l') l = v ==> v <> NONE
 Proof
   rpt strip_tac
   \\ qspecl_then [‘(λ x. ~MEM x l')’, ‘l’] strip_assume_tac FIND_exists
   \\ fs[]
   \\ qspecl_then [‘l’, ‘l'’] imp_res_tac longer_and_distinct_exists
-  \\ qpat_x_assum ‘_ ⇒ _’ imp_res_tac
+  \\ qpat_x_assum ‘_ ==> _’ imp_res_tac
 QED
 
 Theorem generate_unique_name_some:
-  ∀ identifiers base v. generate_unique_name identifiers base = v ⇒ ∃ x. v = SOME x
+  ! identifiers base v. generate_unique_name identifiers base = v ==> ? x. v = SOME x
 Proof
   fs[generate_unique_name_def]
   \\ rpt strip_tac
@@ -1819,7 +1815,7 @@ Proof
 QED
 
 Theorem FIND_result_fulfills:
-  ∀ P l v. FIND P l = SOME v ⇒ P v
+  ! P l v. FIND P l = SOME v ==> P v
 Proof
   Induct_on ‘l’ \\ fs[]
   \\ fs[FIND_thm]
@@ -1828,7 +1824,7 @@ Proof
 QED
 
 Theorem generate_unique_name_is_unique:
-  ∀ identifiers base v. generate_unique_name identifiers base = SOME v ⇒ ~ MEM v identifiers
+  ! identifiers base v. generate_unique_name identifiers base = SOME v ==> ~ MEM v identifiers
 Proof
   fs[generate_unique_name_def]
   \\ rpt strip_tac
@@ -1839,8 +1835,8 @@ Proof
 QED
 
 Triviality v_size_ALOOKUP:
-  ∀ ls n v.
-  ALOOKUP ls n = SOME v ⇒
+  ! ls n v.
+  ALOOKUP ls n = SOME v ==>
   v_size v + 1 < v3_size ls + c
 Proof
   Induct_on ‘ls’ \\ fs[ALOOKUP_def]
@@ -1852,8 +1848,8 @@ Proof
 QED
 
 Triviality v2_size_ALOOKUP:
-  ∀ ls s env.
-  ALOOKUP ls s = SOME env ⇒
+  ! ls s env.
+  ALOOKUP ls s = SOME env ==>
   v2_size env < v4_size ls + c
 Proof
   Induct_on ‘ls’ \\ fs[ALOOKUP_def]
@@ -1865,8 +1861,8 @@ Proof
 QED
 
 Theorem env_size_decreasing:
-  ∀ env x v.
-  nsLookup env x = SOME v ⇒
+  ! env x v.
+  nsLookup env x = SOME v ==>
   v_size v + 1 < v2_size env
 Proof
   ho_match_mp_tac namespaceTheory.nsLookup_ind
@@ -1879,23 +1875,23 @@ Proof
 QED
 
 Definition v_sim_def[simp]:
-  (v_sim [] [] ⇔ T)∧
-  (v_sim (x1::y1::z1) (x2::y2::z2) ⇔ (v_sim [x1] [x2] ∧ v_sim (y1::z1) (y2::z2))) ∧
-  (v_sim [FP_WordTree fp1] [FP_WordTree fp2] ⇔ compress_word fp1 = compress_word fp2)∧
-  (v_sim [FP_BoolTree fp1] [FP_BoolTree fp2] ⇔ compress_bool fp1 = compress_bool fp2)∧
-  (v_sim [Conv ts1 vs1] [Conv ts2 vs2] ⇔ (ts1 = ts2) ∧ v_sim vs1 vs2 )∧
-  (v_sim [Vectorv vs1] [Vectorv vs2] ⇔ v_sim vs1 vs2 )∧
-  (v_sim [Closure env s e] [Closure env2 s2 e2] ⇔ e = e2 ∧ s = s2 ∧ env_sim (env.v) (env2.v)) ∧
-  (v_sim [Recclosure env1 defs1 n1] [Recclosure env2 defs2 n2] ⇔
-            defs1 = defs2 ∧ n1 = n2 ∧ env_sim (env1.v) (env2.v)) ∧
-  (v_sim v1 v2 ⇔  v1 = v2)
-  ∧
+  (v_sim [] [] <=> T)/\
+  (v_sim (x1::y1::z1) (x2::y2::z2) <=> (v_sim [x1] [x2] /\ v_sim (y1::z1) (y2::z2))) /\
+  (v_sim [FP_WordTree fp1] [FP_WordTree fp2] <=> compress_word fp1 = compress_word fp2)/\
+  (v_sim [FP_BoolTree fp1] [FP_BoolTree fp2] <=> compress_bool fp1 = compress_bool fp2)/\
+  (v_sim [Conv ts1 vs1] [Conv ts2 vs2] <=> (ts1 = ts2) /\ v_sim vs1 vs2 )/\
+  (v_sim [Vectorv vs1] [Vectorv vs2] <=> v_sim vs1 vs2 )/\
+  (v_sim [Closure env s e] [Closure env2 s2 e2] <=> e = e2 /\ s = s2 /\ env_sim (env.v) (env2.v)) /\
+  (v_sim [Recclosure env1 defs1 n1] [Recclosure env2 defs2 n2] <=>
+            defs1 = defs2 /\ n1 = n2 /\ env_sim (env1.v) (env2.v)) /\
+  (v_sim v1 v2 <=>  v1 = v2)
+  /\
   env_sim env1 env2 =
-    ((∀ (x:(string,string) id) v1.
-      nsLookup env1 x = SOME v1 ⇒
-      ∃ v2. nsLookup env2 x = SOME v2 ∧
-      v_sim [v1] [v2]) ∧
-    (∀ x. nsLookup env1 x = NONE ⇒ nsLookup env2 x = NONE))
+    ((! (x:(string,string) id) v1.
+      nsLookup env1 x = SOME v1 ==>
+      ? v2. nsLookup env2 x = SOME v2 /\
+      v_sim [v1] [v2]) /\
+    (! x. nsLookup env1 x = NONE ==> nsLookup env2 x = NONE))
 Termination
   wf_rel_tac ‘measure (λ x. case x of | INR p => ((v2_size o FST) p)+2 | INL p => (v7_size o FST) p)’
   \\ fs[] \\ conj_tac
@@ -1910,52 +1906,52 @@ End
 val v_sim_ind = theorem"v_sim_ind";
 
 Definition v_sim1_def[simp]:
-  (v_sim1 (FP_WordTree fp1) (FP_WordTree fp2) ⇔ compress_word fp1 = compress_word fp2)∧
-  (v_sim1 (FP_BoolTree fp1) (FP_BoolTree fp2) ⇔ compress_bool fp1 = compress_bool fp2)∧
-  (v_sim1 (Conv ts1 vs1) (Conv ts2 vs2) ⇔ (ts1 = ts2) ∧ v_sim vs1 vs2 )∧
-  (v_sim1 (Vectorv vs1) (Vectorv vs2) ⇔ v_sim vs1 vs2 ) ∧
-  (v_sim1 (Closure env s e) (Closure env2 s2 e2) ⇔ e = e2 ∧ s = s2 ∧ env_sim (env.v) (env2.v)) ∧
-  (v_sim1 (Recclosure env1 defs1 n1) (Recclosure env2 defs2 n2) ⇔
-            defs1 = defs2 ∧ n1 = n2 ∧ env_sim (env1.v) (env2.v)) ∧
-  (v_sim1 v1 v2 ⇔ (v1 = v2))
+  (v_sim1 (FP_WordTree fp1) (FP_WordTree fp2) <=> compress_word fp1 = compress_word fp2)/\
+  (v_sim1 (FP_BoolTree fp1) (FP_BoolTree fp2) <=> compress_bool fp1 = compress_bool fp2)/\
+  (v_sim1 (Conv ts1 vs1) (Conv ts2 vs2) <=> (ts1 = ts2) /\ v_sim vs1 vs2 )/\
+  (v_sim1 (Vectorv vs1) (Vectorv vs2) <=> v_sim vs1 vs2 ) /\
+  (v_sim1 (Closure env s e) (Closure env2 s2 e2) <=> e = e2 /\ s = s2 /\ env_sim (env.v) (env2.v)) /\
+  (v_sim1 (Recclosure env1 defs1 n1) (Recclosure env2 defs2 n2) <=>
+            defs1 = defs2 /\ n1 = n2 /\ env_sim (env1.v) (env2.v)) /\
+  (v_sim1 v1 v2 <=> (v1 = v2))
 End
 
 Theorem v_sim_LIST_REL:
-  (∀v1 v2. v_sim v1 v2 ⇔ LIST_REL v_sim1 v1 v2) ∧
-  (∀ env1 env2. env_sim env1 env2 ⇒ T)
+  (!v1 v2. v_sim v1 v2 <=> LIST_REL v_sim1 v1 v2) /\
+  (! env1 env2. env_sim env1 env2 ==> T)
 Proof
   ho_match_mp_tac v_sim_ind \\ rw[] \\ Cases_on`v6` \\ rw[]
 QED
 
 Theorem v_sim_empty_r:
-  ∀ xs ys. v_sim xs ys ∧ ys = [] ⇒ xs = []
+  ! xs ys. v_sim xs ys /\ ys = [] ==> xs = []
 Proof
   rw[v_sim_LIST_REL] \\ fs[]
 QED
 
 Theorem v_sim_empty_l:
-  ∀ xs ys. v_sim xs ys ∧ xs = [] ⇒ ys = []
+  ! xs ys. v_sim xs ys /\ xs = [] ==> ys = []
 Proof
   rw[v_sim_LIST_REL] \\ fs[]
 QED
 
 Definition noopt_sim_def[simp]:
-  noopt_sim (Rerr (Rraise v1)) (Rerr (Rraise v2)) = v_sim1 v1 v2 ∧
-  noopt_sim ((Rerr e1):(v list, v) semanticPrimitives$result) v2 = (v2 = Rerr e1) ∧
-  noopt_sim (Rval vs1) (Rval vs2) = v_sim vs1 vs2 ∧
+  noopt_sim (Rerr (Rraise v1)) (Rerr (Rraise v2)) = v_sim1 v1 v2 /\
+  noopt_sim ((Rerr e1):(v list, v) semanticPrimitives$result) v2 = (v2 = Rerr e1) /\
+  noopt_sim (Rval vs1) (Rval vs2) = v_sim vs1 vs2 /\
   noopt_sim _ _ = F
 End
 
 Theorem noopt_sim_val[simp]:
-  noopt_sim (Rval vs1) v2 ⇒
-  ∃ vs2. v2 = Rval vs2
+  noopt_sim (Rval vs1) v2 ==>
+  ? vs2. v2 = Rval vs2
 Proof
   Cases_on ‘v2’ \\ simp[noopt_sim_def]
 QED
 
 Theorem noopt_sim_val_fp[simp]:
-  noopt_sim (Rval [FP_WordTree fp1]) (Rval vs2) ⇒
-  ∃ fp2. vs2 = [FP_WordTree fp2] ∧ compress_word fp1 = compress_word fp2
+  noopt_sim (Rval [FP_WordTree fp1]) (Rval vs2) ==>
+  ? fp2. vs2 = [FP_WordTree fp2] /\ compress_word fp1 = compress_word fp2
 Proof
   simp[noopt_sim_def]
   \\ Cases_on`vs2` \\ simp[]
@@ -1964,23 +1960,23 @@ Proof
 QED
 
 Theorem v_sim_cons:
-  v_sim (x::xs) (y::ys) ⇔ v_sim [x] [y] ∧ v_sim xs ys
+  v_sim (x::xs) (y::ys) <=> v_sim [x] [y] /\ v_sim xs ys
 Proof
   rw[v_sim_LIST_REL]
 QED
 
 Theorem v_sim_refl[simp]:
-  ∀ vs. v_sim vs vs ∧ ∀ env. env_sim env env
+  ! vs. v_sim vs vs /\ ! env. env_sim env env
 Proof
-  `(∀vs1 vs2. vs1 = vs2 ⇒ v_sim vs1 vs2) ∧ (∀ env1 env2. env1 = env2 ⇒ env_sim env1 env2)` suffices_by rw[]
+  `(!vs1 vs2. vs1 = vs2 ==> v_sim vs1 vs2) /\ (! env1 env2. env1 = env2 ==> env_sim env1 env2)` suffices_by rw[]
   \\ ho_match_mp_tac v_sim_ind \\ rw[]
   \\ res_tac \\ fs[]
 QED
 
 Theorem v_sim1_refl[simp]:
-  ∀v. v_sim1 v v
+  !v. v_sim1 v v
 Proof
-  `∀v1 v2. (v1 = v2) ⇒ v_sim1 v1 v2` suffices_by rw[]
+  `!v1 v2. (v1 = v2) ==> v_sim1 v1 v2` suffices_by rw[]
   \\ recInduct v_sim1_ind \\ rw[]
 QED
 
@@ -1992,19 +1988,19 @@ Proof
 QED
 
 Theorem noopt_sim_rerr_rval[simp]:
-  ¬noopt_sim (Rerr x) (Rval y) ∧
-  ¬noopt_sim (Rval z) (Rerr w)
+  ~noopt_sim (Rerr x) (Rval y) /\
+  ~noopt_sim (Rval z) (Rerr w)
 Proof
   Cases_on`x` \\ Cases_on`w` \\ simp[]
 QED
 
 Theorem v_sim_fpoptimise:
-  (∀ vs1 vs2.
-  v_sim vs1 vs2 ⇒
+  (! vs1 vs2.
+  v_sim vs1 vs2 ==>
   v_sim (do_fpoptimise annot1 vs1) (do_fpoptimise annot2 vs2))
-  ∧
-  (∀ env1 env2.
-   env_sim env1 env2 ⇒ T)
+  /\
+  (! env1 env2.
+   env_sim env1 env2 ==> T)
 Proof
   ho_match_mp_tac v_sim_ind
   \\ fs[v_sim_def, do_fpoptimise_def, fpSemTheory.compress_word_def, fpSemTheory.compress_bool_def]
@@ -2012,9 +2008,9 @@ Proof
 QED
 
 Theorem do_log_v_sim1:
-  ∀v1 v2.
-  v_sim1 v1 v2 ⇒
-  ∀ e1 e2.
+  !v1 v2.
+  v_sim1 v1 v2 ==>
+  ! e1 e2.
     do_log l v2 e2 =
     case do_log l v1 e1 of
     | NONE => NONE
@@ -2029,20 +2025,20 @@ Proof
 QED
 
 Theorem pmatch_v_sim1:
-  (∀envC refs p v env.
-     ∀v2 env2.  v_sim1 v v2 ∧ MAP FST env = MAP FST env2 ∧ v_sim (MAP SND env) (MAP SND env2)  ⇒
+  (!envC refs p v env.
+     !v2 env2.  v_sim1 v v2 /\ MAP FST env = MAP FST env2 /\ v_sim (MAP SND env) (MAP SND env2)  ==>
      case pmatch envC refs p v env of
      | Match_type_error => pmatch envC refs p v2 env2 = Match_type_error
      | No_match => pmatch envC refs p v2 env2 = No_match
-     | Match env3 => ∃env4. pmatch envC refs p v2 env2 = Match env4 ∧
-                            MAP FST env3 = MAP FST env4 ∧ v_sim (MAP SND env3) (MAP SND env4)) ∧
-  (∀envC refs ps vs env.
-     ∀vs2 env2. v_sim vs vs2 ∧ MAP FST env = MAP FST env2 ∧ v_sim (MAP SND env) (MAP SND env2)  ⇒
+     | Match env3 => ?env4. pmatch envC refs p v2 env2 = Match env4 /\
+                            MAP FST env3 = MAP FST env4 /\ v_sim (MAP SND env3) (MAP SND env4)) /\
+  (!envC refs ps vs env.
+     !vs2 env2. v_sim vs vs2 /\ MAP FST env = MAP FST env2 /\ v_sim (MAP SND env) (MAP SND env2)  ==>
      case pmatch_list envC refs ps vs env of
      | Match_type_error => pmatch_list envC refs ps vs2 env2 = Match_type_error
      | No_match => pmatch_list envC refs ps vs2 env2 = No_match
-     | Match env3 => ∃env4. pmatch_list envC refs ps vs2 env2 = Match env4 ∧
-                            MAP FST env3 = MAP FST env4 ∧ v_sim (MAP SND env3) (MAP SND env4))
+     | Match env3 => ?env4. pmatch_list envC refs ps vs2 env2 = Match env4 /\
+                            MAP FST env3 = MAP FST env4 /\ v_sim (MAP SND env3) (MAP SND env4))
 Proof
   ho_match_mp_tac pmatch_ind
   \\  rw[pmatch_def] \\  rw[pmatch_def]
@@ -2056,8 +2052,8 @@ Proof
 QED
 
 Theorem can_pmatch_all_v_sim1:
-  ∀envC refs ps v1 v2.
-    v_sim1 v1 v2 ⇒
+  !envC refs ps v1 v2.
+    v_sim1 v1 v2 ==>
       can_pmatch_all envC refs ps v1 = can_pmatch_all envC refs ps v2
 Proof
   Induct_on`ps`
@@ -2072,10 +2068,10 @@ QED
 val _ = augment_srw_ss[rewrites[fp_translate_def]];
 
 Theorem fp_translate_v_sim1:
-  v_sim1 v1 v2 ⇒
+  v_sim1 v1 v2 ==>
     case fp_translate v1 of
     | NONE => fp_translate v2 = NONE
-    | SOME w1 => ∃w2. fp_translate v2 = SOME w2 ∧ v_sim1 w1 w2
+    | SOME w1 => ?w2. fp_translate v2 = SOME w2 /\ v_sim1 w1 w2
 Proof
   Cases_on`v1` \\ Cases_on`v2` \\ rw[]
   \\ Cases_on`l` \\ rw[]
@@ -2083,18 +2079,18 @@ QED
 
 (* TODO: move *)
 Theorem do_eq_refl:
-  (∀v1 v2.  v1 = v2 ⇒ do_eq v1 v2 = Eq_val T) ∧
-  (∀v1 v2 .  v1 = v2 ⇒ do_eq_list v1 v2 = Eq_val T)
+  (!v1 v2.  v1 = v2 ==> do_eq v1 v2 = Eq_val T) /\
+  (!v1 v2 .  v1 = v2 ==> do_eq_list v1 v2 = Eq_val T)
 Proof
   ho_match_mp_tac do_eq_ind \\ rw[do_eq_def]
 QED
 
 Theorem do_eq_v_sim1:
-  (∀v1 v2 v3 v4.
-     v_sim1 v1 v2 ∧ v_sim1 v3 v4 ⇒
-       do_eq v1 v3 = do_eq v2 v4) ∧
-  (∀v1 v2 v3 v4.
-    v_sim v1 v2 ∧ v_sim v3 v4 ⇒
+  (!v1 v2 v3 v4.
+     v_sim1 v1 v2 /\ v_sim1 v3 v4 ==>
+       do_eq v1 v3 = do_eq v2 v4) /\
+  (!v1 v2 v3 v4.
+    v_sim v1 v2 /\ v_sim v3 v4 ==>
       do_eq_list v1 v3 = do_eq_list v2 v4)
 Proof
   ho_match_mp_tac do_eq_ind \\ rw[do_eq_def]
@@ -2114,7 +2110,7 @@ Proof
 QED
 
 Theorem v_to_char_list_v_sim1:
-  ∀x y. v_sim1 x y ⇒ v_to_char_list x = v_to_char_list y
+  !x y. v_sim1 x y ==> v_to_char_list x = v_to_char_list y
 Proof
   recInduct v_to_char_list_ind
   \\ rw[v_to_char_list_def]
@@ -2132,10 +2128,10 @@ Proof
 QED
 
 Theorem v_to_list_v_sim1:
-  ∀x y. v_sim1 x y ⇒
+  !x y. v_sim1 x y ==>
     case v_to_list x of
     NONE => v_to_list y = NONE
-    | SOME v2 => ∃v3. v_to_list y = SOME v3 ∧ v_sim v2 v3
+    | SOME v2 => ?v3. v_to_list y = SOME v3 /\ v_sim v2 v3
 Proof
   recInduct v_to_list_ind
   \\ rw[v_to_list_def]
@@ -2149,7 +2145,7 @@ Proof
 QED
 
 Theorem vs_to_string_v_sim:
-  ∀x y. v_sim x y ⇒ vs_to_string x = vs_to_string y
+  !x y. v_sim x y ==> vs_to_string x = vs_to_string y
 Proof
   recInduct vs_to_string_ind
   \\ rw[vs_to_string_def]
@@ -2161,9 +2157,9 @@ Proof
 QED
 
 Theorem list_to_v_v_sim1:
-  ∀l1 l2.
+  !l1 l2.
   v_sim l1 l2
-  ⇒
+  ==>
   v_sim1 (list_to_v l1) (list_to_v l2)
 Proof
   Induct \\ rw[list_to_v_def]
@@ -2183,13 +2179,13 @@ QED
 val _ = augment_srw_ss[rewrites[sv_rel_v_sim1_refl]];
 
 Theorem do_app_v_sim:
-  v_sim v1 v2 ⇒
+  v_sim v1 v2 ==>
     case do_app x op v1 of
     | NONE => do_app x op v2 = NONE
     | SOME ((sv1, y), r1) =>
-      ∃ sv2 r2.
-        do_app x op v2 = SOME ((sv2, y), r2) ∧
-        LIST_REL (sv_rel v_sim1) sv1 sv2 ∧ (isPureOp op ⇒ sv1 = sv2) ∧
+      ? sv2 r2.
+        do_app x op v2 = SOME ((sv2, y), r2) /\
+        LIST_REL (sv_rel v_sim1) sv1 sv2 /\ (isPureOp op ==> sv1 = sv2) /\
         noopt_sim (list_result r1) (list_result r2)
 Proof
   rw[v_sim_LIST_REL]
@@ -2320,7 +2316,7 @@ Proof
 QED
 
 Theorem build_conv_v_sim:
-  v_sim v1 v2 ⇒  OPTREL v_sim1 (build_conv envc x v1 ) (build_conv envc x v2)
+  v_sim v1 v2 ==>  OPTREL v_sim1 (build_conv envc x v1 ) (build_conv envc x v2)
 Proof
   rw[build_conv_def]
   \\ TOP_CASE_TAC \\ simp[OPTREL_def]
@@ -2333,18 +2329,18 @@ local
   (* exp goal *)
   val P0 =
   “λ (e:ast$exp).
-   ∀ st env cfg st2 r choices fpScope.
-   evaluate st env [no_optimisations cfg e] = (st2, r) ∧
-   st.fp_state.canOpt ≠ FPScope Opt ∧
-   isPureExp e ⇒
-     ∀ env2.
-       env_sim (env.v) env2 ⇒
-       ∃ choices2 r2.
+   ! st env cfg st2 r choices fpScope.
+   evaluate st env [no_optimisations cfg e] = (st2, r) /\
+   st.fp_state.canOpt <> FPScope Opt /\
+   isPureExp e ==>
+     ! env2.
+       env_sim (env.v) env2 ==>
+       ? choices2 r2.
          evaluate
            (st with fp_state :=
             st.fp_state with <| opts := (λ x. []); rws := []; canOpt:= FPScope fpScope; choices := choices |>)
         (env with v := env2) [e] =
-        (st2 with fp_state := st.fp_state with <| opts := (λ x. []); rws := []; canOpt:= FPScope fpScope; choices := choices2|>, r2) ∧ noopt_sim r r2”
+        (st2 with fp_state := st.fp_state with <| opts := (λ x. []); rws := []; canOpt:= FPScope fpScope; choices := choices2|>, r2) /\ noopt_sim r r2”
   (* P4: string * exp -> bool *)
   val P4 =
   Parse.Term (‘λ (s:string, e). ^P0 e’);
@@ -2354,47 +2350,47 @@ local
   (* Letrec goal *)
   val P1 =
   Parse.Term (‘λ (l:(string # string # exp) list).
-  ∀ p. MEM p l ⇒ ^P2 p’)
+  ! p. MEM p l ==> ^P2 p’)
   (* P5: pat * exp -> bool *)
   val P5 =
   Parse.Term (‘λ (p:pat, e). ^P0 e’)
   (* P3: pat * exp list -> bool *)
   val P3 =
   Parse.Term (‘λ (pes:(pat # exp) list).
-  ∀ st env v cfg err_v st2 r cfg choices fpScope.
-  evaluate_match st env v (MAP (λ (p,e). (p, no_optimisations cfg e)) pes) err_v = (st2, r) ∧
-  st.fp_state.canOpt ≠ FPScope Opt ∧
-  isPurePatExpList pes ⇒
-    ∀ env2 v2 err_v2. env_sim env.v env2 ∧ v_sim1 v v2 ∧ v_sim1 err_v err_v2 ⇒
-    ∃ choices2 r2.
+  ! st env v cfg err_v st2 r cfg choices fpScope.
+  evaluate_match st env v (MAP (λ (p,e). (p, no_optimisations cfg e)) pes) err_v = (st2, r) /\
+  st.fp_state.canOpt <> FPScope Opt /\
+  isPurePatExpList pes ==>
+    ! env2 v2 err_v2. env_sim env.v env2 /\ v_sim1 v v2 /\ v_sim1 err_v err_v2 ==>
+    ? choices2 r2.
       evaluate_match
         (st with fp_state :=
           st.fp_state with <| opts := (λ x. []); rws := []; canOpt:= FPScope fpScope; choices := choices|>)
       (env with v := env2) v2 pes err_v2 =
-        (st2 with fp_state := st.fp_state with <| opts := (λ x. []); rws := []; canOpt:= FPScope fpScope; choices := choices2|>, r2) ∧ noopt_sim r r2’);
+        (st2 with fp_state := st.fp_state with <| opts := (λ x. []); rws := []; canOpt:= FPScope fpScope; choices := choices2|>, r2) /\ noopt_sim r r2’);
   (* P6: exp list -> bool *)
   val P6 =
-    Parse.Term (‘λ (es:ast$exp list). ∀ e. MEM e es ⇒ ^P0 e’);
+    Parse.Term (‘λ (es:ast$exp list). ! e. MEM e es ==> ^P0 e’);
   val ind_thm =
     astTheory.exp_induction |> SPEC P0 |> SPEC P1 |> SPEC P2 |> SPEC P3
     |> SPEC P4 |> SPEC P5 |> SPEC P6;
 in
 
 Triviality lift_P6_noopt_REVERSE:
-  ∀ es.
-    ^P6 es ⇒
-   ∀ (st:'a semanticPrimitives$state) env cfg st2 r choices fpScope.
-   evaluate st env (MAP (no_optimisations cfg) es) = (st2, r) ∧
-   st.fp_state.canOpt ≠ FPScope Opt ∧
-   isPureExpList es ⇒
-     ∀ env2.
-     env_sim env.v env2 ⇒
-     ∃ choices2 r2.
+  ! es.
+    ^P6 es ==>
+   ! (st:'a semanticPrimitives$state) env cfg st2 r choices fpScope.
+   evaluate st env (MAP (no_optimisations cfg) es) = (st2, r) /\
+   st.fp_state.canOpt <> FPScope Opt /\
+   isPureExpList es ==>
+     ! env2.
+     env_sim env.v env2 ==>
+     ? choices2 r2.
        evaluate
          (st with fp_state :=
           st.fp_state with <| opts := (λ x. []); rws := []; canOpt:= FPScope fpScope; choices := choices |>)
         (env with v := env2) es =
-        (st2 with fp_state := st.fp_state with <| opts := (λ x. []); rws := []; canOpt:= FPScope fpScope; choices := choices2|>, r2) ∧
+        (st2 with fp_state := st.fp_state with <| opts := (λ x. []); rws := []; canOpt:= FPScope fpScope; choices := choices2|>, r2) /\
         noopt_sim r r2
 Proof
   Induct \\ fs[]
@@ -2414,7 +2410,7 @@ Proof
   \\ fs[CaseEq"prod"]
   \\ first_x_assum (first_assum o mp_then Any (qspecl_then[`choices2`, `fpScope`]strip_assume_tac))
   \\ ntac 2 (first_x_assum (first_assum o mp_then Any assume_tac)) \\ fs[]
-  \\ ‘s'.fp_state.canOpt ≠ FPScope Opt’ by (imp_res_tac evaluate_fp_opts_inv \\ fs[])
+  \\ ‘s'.fp_state.canOpt <> FPScope Opt’ by (imp_res_tac evaluate_fp_opts_inv \\ fs[])
   \\ fs[]
   \\ qmatch_asmsub_abbrev_tac`evaluate s1 envA es`
   \\ qmatch_goalsub_abbrev_tac`evaluate s11 envA es`
@@ -2430,8 +2426,8 @@ Proof
 QED
 
 Theorem no_optimisations_backwards_sim:
-  (∀ e. ^P0 e) ∧ (∀ l. ^P1 l) ∧ (∀ p. ^P2 p) ∧ (∀ l. ^P3 l) ∧ (∀ p. ^P4 p)
-  ∧ (∀ p. ^P5 p) ∧ (∀ l. ^P6 l)
+  (! e. ^P0 e) /\ (! l. ^P1 l) /\ (! p. ^P2 p) /\ (! l. ^P3 l) /\ (! p. ^P4 p)
+  /\ (! p. ^P5 p) /\ (! l. ^P6 l)
 Proof
   irule ind_thm \\ rpt strip_tac \\ fs[]
   \\ rpt strip_tac
@@ -2455,7 +2451,7 @@ Proof
    >- (
     rpt strip_tac
     \\ Cases_on ‘v’ \\ fs[v_sim1_def] \\ rveq
-    \\ ‘q.fp_state.canOpt ≠ FPScope Opt’ by (imp_res_tac evaluate_fp_opts_inv \\ fs[])
+    \\ ‘q.fp_state.canOpt <> FPScope Opt’ by (imp_res_tac evaluate_fp_opts_inv \\ fs[])
     \\ res_tac
     \\ rpt (first_x_assum (qspecl_then [‘fpScope’, ‘choices2’] assume_tac))
     \\ fs[evaluate_def, fpState_component_equality, semState_comp_eq,
@@ -2481,7 +2477,7 @@ Proof
     \\ fs[fpState_component_equality, semState_comp_eq])
     \\ rpt strip_tac
     \\ Cases_on ‘v’ \\ fs[v_sim1_def] \\ rveq
-    \\ ‘q.fp_state.canOpt ≠ FPScope Opt’ by (imp_res_tac evaluate_fp_opts_inv \\ fs[])
+    \\ ‘q.fp_state.canOpt <> FPScope Opt’ by (imp_res_tac evaluate_fp_opts_inv \\ fs[])
     \\ res_tac
     \\ rpt (first_x_assum (qspecl_then [‘fpScope’, ‘choices2’] assume_tac))
     \\ fs[evaluate_def, fpState_component_equality, semState_comp_eq,
@@ -2501,7 +2497,7 @@ Proof
     \\ pop_assum (first_assum o mp_then Any strip_assume_tac)
     \\ simp[Once evaluate_def]
     \\ reverse(fs[CaseEq"result"] \\ rveq \\ fs[noopt_sim_def])
-    \\ ‘st.fp_state.canOpt ≠ FPScope Opt’ by (imp_res_tac evaluate_fp_opts_inv \\ fs[])
+    \\ ‘st.fp_state.canOpt <> FPScope Opt’ by (imp_res_tac evaluate_fp_opts_inv \\ fs[])
     \\ fs[]
     \\ Cases_on`r2` \\ fs[noopt_sim_def]
     >- rw[semState_comp_eq, fpState_component_equality]
@@ -2529,7 +2525,7 @@ Proof
     \\ ntac 2 (pop_assum (first_assum o mp_then Any strip_assume_tac))
     \\ simp[Once evaluate_def]
     \\ reverse(fs[CaseEq"result"] \\ rveq \\ fs[noopt_sim_def])
-    \\ ‘st.fp_state.canOpt ≠ FPScope Opt’ by (imp_res_tac evaluate_fp_opts_inv \\ fs[])
+    \\ ‘st.fp_state.canOpt <> FPScope Opt’ by (imp_res_tac evaluate_fp_opts_inv \\ fs[])
     \\ fs[]
     \\ Cases_on`r2` \\ fs[noopt_sim_def]
     >- rw[semState_comp_eq, fpState_component_equality]
@@ -2592,7 +2588,7 @@ Proof
     \\ first_x_assum (first_x_assum o mp_then Any (qspecl_then[`choices`,`fpScope`,`env2`]mp_tac))
     \\ impl_tac >- simp[] \\ strip_tac
     \\ reverse(fs[CaseEq"result", CaseEq"error_result"] \\ rveq \\ fs[noopt_sim_def])
-    \\ ‘st.fp_state.canOpt ≠ FPScope Opt’ by (imp_res_tac evaluate_fp_opts_inv \\ fs[])
+    \\ ‘st.fp_state.canOpt <> FPScope Opt’ by (imp_res_tac evaluate_fp_opts_inv \\ fs[])
     \\ fs[]
     \\ Cases_on`r2` \\ fs[noopt_sim_def]
     >- rw[semState_comp_eq, fpState_component_equality]
@@ -2692,7 +2688,7 @@ Proof
     >- ( rw[semState_comp_eq, fpState_component_equality] )
     \\ fs[CaseEq"prod"] \\ strip_tac \\ fs[]
     \\ rveq \\ fs[]
-    \\ ‘st'.fp_state.canOpt ≠ FPScope Opt’ by (imp_res_tac evaluate_fp_opts_inv \\ fs[])
+    \\ ‘st'.fp_state.canOpt <> FPScope Opt’ by (imp_res_tac evaluate_fp_opts_inv \\ fs[])
     \\ fs[]
     \\ Cases_on ‘fpScope = Opt’
     \\ fs[do_fprw_def, rwAllWordTree_def, rwAllBoolTree_def, shift_fp_opts_def,
@@ -2763,9 +2759,9 @@ Proof
         fs[isPureExp_def]
         \\ qmatch_assum_rename_tac`MAP FST env1 = MAP FST env4`
         \\ qmatch_goalsub_abbrev_tac `nsLookup env11`
-        \\ `∀x. case nsLookup env11 x  of
+        \\ `!x. case nsLookup env11 x  of
                 | NONE => nsLookup env22 x = NONE
-                | SOME v1 => ∃v2. nsLookup env22 x = SOME v2 ∧ v_sim1 v1 v2` suffices_by (
+                | SOME v1 => ?v2. nsLookup env22 x = SOME v2 /\ v_sim1 v1 v2` suffices_by (
               rw[]
               \\ first_x_assum(qspec_then`x`mp_tac) \\ rw[]
               \\ rw[v_sim_LIST_REL] )
@@ -2776,7 +2772,7 @@ Proof
         \\ TRY (Cases_on`p1` \\ fs[namespacePropsTheory.nsLookupMod_alist_to_ns] \\ NO_TAC)
         >- (
           rw[]
-          \\ `∀x. MEM x (MAP FST env1) = MEM x (MAP FST env4)` by simp[]
+          \\ `!x. MEM x (MAP FST env1) = MEM x (MAP FST env4)` by simp[]
           \\ fs[MEM_MAP, EXISTS_PROD]
           \\ metis_tac[] )
         \\ reverse(fs[namespacePropsTheory.nsLookup_nsAppend_some])
@@ -2790,7 +2786,7 @@ Proof
           \\ conj_tac
           >- (
             fs[ALOOKUP_FAILS]
-            \\ `∀x. MEM x (MAP FST env1) = MEM x (MAP FST env4)` by simp[]
+            \\ `!x. MEM x (MAP FST env1) = MEM x (MAP FST env4)` by simp[]
             \\ fs[MEM_MAP, EXISTS_PROD]
             \\ metis_tac[] )
           \\ Cases \\ simp[] )
@@ -2827,17 +2823,17 @@ Theorem no_optimisations_eval_sim =
   |> GEN_ALL ;
 
 Theorem do_foptimise_cons:
-  ∀y x .
+  !y x .
   do_fpoptimise f (x::y) = (do_fpoptimise f [x]) ++ (do_fpoptimise f y)
 Proof
   Induct>>EVAL_TAC>>simp[]
 QED
 
 Theorem evaluate_no_optimisations:
-  ∀ fpScope choices.
-  evaluate st env [realify (no_optimisations cfg e)] = (st, Rval [Real r]) ∧
-  (st.fp_state.canOpt ≠ FPScope Opt ∧ isPureExp e) ⇒
-  ∃ st2.
+  ! fpScope choices.
+  evaluate st env [realify (no_optimisations cfg e)] = (st, Rval [Real r]) /\
+  (st.fp_state.canOpt <> FPScope Opt /\ isPureExp e) ==>
+  ? st2.
     evaluate
       (st with fp_state := st.fp_state with
          <| rws := []; opts := (λ x. []); choices:= choices; canOpt := FPScope fpScope|>)
@@ -2856,36 +2852,37 @@ Proof
 QED
 
 Inductive res_sim:
-  (∀ (e1:v error_result) (e2:v error_result) (cfg:config) (st1:'a semanticPrimitives$state).
+  (! (e1:v error_result) (e2:v error_result) (cfg:config) (st1:'a semanticPrimitives$state).
    res_sim (Rerr e1) (Rerr e2) cfg st1)
-  ∧
-  (∀ (vs1:v list) (vs2:v list) (cfg:config) (st1:'a semanticPrimitives$state).
-   v_list_sim vs1 vs2 cfg st1 ⇒
+  /\
+  (! (vs1:v list) (vs2:v list) (cfg:config) (st1:'a semanticPrimitives$state).
+   v_list_sim vs1 vs2 cfg st1 ==>
    res_sim (Rval vs1) (Rval vs2) cfg st1)
-  ∧
-  (∀ (cfg:config) (st1:'a semanticPrimitives$state).
-   v_list_sim [] [] cfg st1) ∧
-  (∀ v1 v2 vs1 vs2 cfg st1 .
-   v_list_sim vs1 vs2 cfg st1 ∧
-   v1 = v2 ⇒
+  /\
+  (! (cfg:config) (st1:'a semanticPrimitives$state).
+   v_list_sim [] [] cfg st1) /\
+  (! v1 v2 vs1 vs2 cfg st1 .
+   v_list_sim vs1 vs2 cfg st1 /\
+   v1 = v2 ==>
    v_list_sim (v1::vs1) (v2::vs2) cfg st1)
-  ∧
-  (∀ v1 v2 vs1 vs2 cfg env s e (st1:'a semanticPrimitives$state).
-   v_list_sim vs1 vs2 cfg st1 ∧
-   v2 = Closure env s e ∧
-   v1 = Closure env s (HD(stos_pass cfg [e])) ∧
-   (∀ st r1 (st2:'a semanticPrimitives$state).
-    st1.fp_state.rws = st.fp_state.rws ⇒
-    evaluate st env (stos_pass cfg [e]) = (st2, Rval r1) ∧
-    (cfg.canOpt ⇔ st.fp_state.canOpt = FPScope Opt) ∧
-    (st.fp_state.canOpt ≠ Strict) ∧
+  /\
+  (! v1 v2 vs1 vs2 cfg env s e (st1:'a semanticPrimitives$state) plan.
+    rws = FLAT (MAP (λ x. case x of |Apply (_, rws) => rws | _ => []) plan) ∧
+   v_list_sim vs1 vs2 cfg st1 /\
+   v2 = Closure env s e /\
+   v1 = Closure env s (FST (HD (stos_pass_with_plans cfg [plan] [e]))) /\
+   (! st r1 (st2:'a semanticPrimitives$state).
+    st1.fp_state.rws = st.fp_state.rws ==>
+    evaluate st env (MAP FST (stos_pass_with_plans cfg [plan] [e])) = (st2, Rval r1) /\
+    (cfg.canOpt <=> st.fp_state.canOpt = FPScope Opt) /\
+    (st.fp_state.canOpt <> Strict) /\
     (~ st.fp_state.real_sem) ==>
-    ∃ fpOpt choices fpOptR choicesR r2.
+    ? fpOpt choices fpOptR choicesR r2.
     (evaluate (st with fp_state := st.fp_state with
-               <| rws := st.fp_state.rws ++ (cfg.optimisations) ; opts := fpOpt; choices := choices |>) env [e] =
+               <| rws := st.fp_state.rws ++ rws ; opts := fpOpt; choices := choices |>) env [e] =
      (st2 with fp_state := st2.fp_state with
-      <| rws := st2.fp_state.rws ++ (cfg.optimisations) ; opts := fpOptR; choices := choicesR |>, Rval r2)) ∧
-    res_sim (Rval r1) (Rval r2) cfg st1) ⇒
+      <| rws := st2.fp_state.rws ++ rws ; opts := fpOptR; choices := choicesR |>, Rval r2)) /\
+    res_sim (Rval r1) (Rval r2) cfg st1) ==>
    v_list_sim (v1::vs1) (v2::vs2) cfg st1)
 End
 
@@ -2909,62 +2906,212 @@ QED
 Definition is_stos_pass_with_plans_correct_def :
   is_stos_pass_with_plans_correct plans (st1:'a semanticPrimitives$state) st2 env cfg exps r1 =
     (evaluate st1 env
-             (MAP FST (stos_pass_with_plans cfg plans exps)) = (st2, Rval r1) ∧
-     (cfg.canOpt ⇔ st1.fp_state.canOpt = FPScope Opt) ∧
-     (st1.fp_state.canOpt ≠ Strict) ∧
+             (MAP FST (stos_pass_with_plans cfg plans exps)) = (st2, Rval r1) /\
+     (cfg.canOpt <=> st1.fp_state.canOpt = FPScope Opt) /\
+     (st1.fp_state.canOpt <> Strict) /\
      (~ st1.fp_state.real_sem) ==>
      let theRws = FLAT (MAP (λ stp. case stp of |Apply (pth, rws) => rws | _ => []) (FLAT plans)) in
-    ∃ fpOpt choices fpOptR choicesR r2.
+    ? fpOpt choices fpOptR choicesR r2.
       (evaluate (st1 with fp_state := st1.fp_state with
                 <| rws := st1.fp_state.rws ++ theRws; opts := fpOpt; choices := choices |>) env exps =
       (st2 with fp_state := st2.fp_state with
-       <| rws := st2.fp_state.rws ++ theRws; opts := fpOptR; choices := choicesR |>, Rval r2)) ∧
-      res_sim (Rval r1) (Rval r2) (cfg with optimisations := theRws) st1)
+       <| rws := st2.fp_state.rws ++ theRws; opts := fpOptR; choices := choicesR |>, Rval r2)) /\
+      res_sim (Rval r1) (Rval r2) cfg st1)
 End
 
-(*
 Theorem res_sim_swap:
-  (∀ vs1 vs2 cfg (st1:'a semanticPrimitives$state).
-  res_sim vs1 vs2 cfg st1 ⇒
-  ∀ (st2:'a semanticPrimitives$state).
-  st1.fp_state.rws = st2.fp_state.rws ∧
-  (st1.fp_state.canOpt = FPScope Opt ⇔ st2.fp_state.canOpt = FPScope Opt) ∧
-  (st1.fp_state.canOpt ≠ Strict) ∧
-  (~ st1.fp_state.real_sem) ⇒
+  (! vs1 vs2 cfg (st1:'a semanticPrimitives$state).
+  res_sim vs1 vs2 cfg st1 ==>
+  ! (st2:'a semanticPrimitives$state).
+  st1.fp_state.rws = st2.fp_state.rws /\
+  (st1.fp_state.canOpt = FPScope Opt <=> st2.fp_state.canOpt = FPScope Opt) /\
+  (st1.fp_state.canOpt <> Strict) /\
+  (~ st1.fp_state.real_sem) ==>
   res_sim vs1 vs2 cfg st2)
-  ∧
-  (∀ vs1 vs2 cfg (st1:'a semanticPrimitives$state).
-  v_list_sim vs1 vs2 cfg st1 ⇒
-  ∀ (st2:'a semanticPrimitives$state).
-  st1.fp_state.rws = st2.fp_state.rws ∧
-  (st1.fp_state.canOpt = FPScope Opt ⇔ st2.fp_state.canOpt = FPScope Opt) ∧
-  (st1.fp_state.canOpt ≠ Strict) ∧
-  (~ st1.fp_state.real_sem) ⇒
+  /\
+  (! vs1 vs2 cfg (st1:'a semanticPrimitives$state).
+  v_list_sim vs1 vs2 cfg st1 ==>
+  ! (st2:'a semanticPrimitives$state).
+  st1.fp_state.rws = st2.fp_state.rws /\
+  (st1.fp_state.canOpt = FPScope Opt <=> st2.fp_state.canOpt = FPScope Opt) /\
+  (st1.fp_state.canOpt <> Strict) /\
+  (~ st1.fp_state.real_sem) ==>
   v_list_sim vs1 vs2 cfg st2)
 Proof
   ho_match_mp_tac res_sim_ind \\ rpt conj_tac \\ rpt strip_tac
-  \\ fs[Once res_sim_cases]
-  >- (
-   first_x_assum (qspec_then ‘st2’ mp_tac)
-   \\ impl_tac \\ fs[]
-   \\ strip_tac \\ rveq \\ fs[Once res_sim_rules])
-  >- (
-   first_x_assum (qspec_then ‘st2’ mp_tac)
-   \\ impl_tac \\ fs[]
-   \\ strip_tac \\ rveq \\ fs[Once res_sim_rules])
-  \\ last_x_assum (qspec_then ‘st2’ mp_tac)
-  \\ impl_tac \\ fs[]
-  \\ strip_tac
-  \\ rveq  \\ fs[Once res_sim_rules] \\ DISJ2_TAC
-  \\ conj_tac \\ fs[Once res_sim_rules]
+  \\ simp[Once res_sim_cases]
+  \\ DISJ2_TAC \\ qexists_tac ‘plan’ \\ fs[]
+  \\ qmatch_goalsub_abbrev_tac ‘FLAT (MAP getRws_from_plan plan)’
   \\ rpt strip_tac
-  \\ res_tac
-  \\ first_x_assum (qspec_then ‘st2’ mp_tac)
-  \\ impl_tac \\ fs[] \\ strip_tac
-  \\ qexists_tac ‘fpOpt'’ \\ qexists_tac ‘choices'’
-  \\ fs[Once res_sim_rules, semState_comp_eq, fpState_component_equality]
+  \\ first_x_assum (qspecl_then [‘st’, ‘r1’, ‘st2'’] mp_tac)
+  \\ impl_tac \\ fs[]
+  \\ strip_tac \\ rveq \\ qexistsl_tac [‘fpOpt’, ‘choices’]
+  \\ fs[semState_comp_eq, fpState_component_equality]
 QED
-*)
+
+Theorem res_sim_refl:
+  res_sim (Rval vs1) (Rval vs1) cfg st
+Proof
+  irule (CONJUNCT1 (CONJUNCT2 res_sim_rules))
+  \\ Induct_on ‘vs1’ \\ fs[res_sim_rules]
+QED
+
+Theorem MAP_FST_Success:
+  MAP FST (MAP (λ e. (e, Success)) exps) = exps
+Proof
+  Induct_on ‘exps’ \\ fs[]
+QED
+
+val simple_case_tac =
+  ntac 4 (TOP_CASE_TAC \\ fs[]) \\ rpt strip_tac
+  \\ rveq \\ fs[MAP_FST_Success]
+  \\ qexistsl_tac [‘st1.fp_state.opts’, ‘st1.fp_state.choices’]
+  \\ qmatch_goalsub_abbrev_tac ‘evaluate st1New _ _’
+  \\ ‘st1New = st1’ by (unabbrev_all_tac \\ fs[semState_comp_eq, fpState_component_equality])
+  \\ rveq \\ simp[Once evaluate_cons]
+  \\ fs[semState_comp_eq, fpState_component_equality, res_sim_refl];
+
+Theorem stos_pass_with_plans_correct_empty:
+  ! exps (st1:'a semanticPrimitives$state) st2 env cfg r.
+   is_stos_pass_with_plans_correct [] st1 st2 env cfg exps r
+Proof
+  Cases_on ‘exps’ \\ rpt strip_tac
+  \\ fs[is_stos_pass_with_plans_correct_def, stos_pass_with_plans_def]
+  >- (
+  rpt strip_tac \\ fs[] \\ rveq
+  \\ fs[res_sim_rules, semState_comp_eq, fpState_component_equality])
+  \\ Cases_on ‘h’ \\ fs[stos_pass_with_plans_def, Once evaluate_cons]
+  \\ simple_case_tac
+QED
+
+Theorem stos_pass_with_plans_sing_exists:
+  ∃ e_opt res. stos_pass_with_plans cfg [h][e] = [(e_opt, res)]
+Proof
+  measureInduct_on ‘exp_size e’\\ Cases_on ‘e’ \\ fs[stos_pass_with_plans_def]
+  \\ TRY (qmatch_goalsub_abbrev_tac ‘optimise_with_plan _ _ (eOld)’
+          \\ Cases_on ‘optimise_with_plan cfg h eOld’ \\ fs[])
+  \\ first_x_assum (qspec_then ‘e'’ mp_tac) \\ fs[astTheory.exp_size_def]
+  \\ strip_tac \\ fs[]
+QED
+
+Theorem MAP_FST_Fun:
+  MAP FST ((λ (e_opt, res). [(Fun s e_opt, res)])(HD (stos_pass_with_plans cfg [h][e]))) =
+  [Fun s (FST (HD (stos_pass_with_plans cfg [h][e])))]
+Proof
+  qspec_then ‘e’ assume_tac (GEN “e:ast$exp”stos_pass_with_plans_sing_exists)
+  \\ fs[]
+QED
+
+val solve_tac =
+  qpat_assum `evaluate _ _ [FST (optimise_with_plan _ _ _)] = _`
+       (fn th => first_x_assum (fn ith => mp_then Any mp_tac ith th))
+  \\ impl_tac \\ fs[]
+  \\ strip_tac \\ pop_assum (mp_then Any mp_tac (CONJUNCT1 evaluate_fp_rws_append))
+  \\ disch_then (qspec_then ‘FLAT_plans’ assume_tac)
+  \\ first_x_assum (qspec_then ‘LENGTH t + exp6_size t'’ mp_tac)
+  \\ impl_tac >- fs[astTheory.exp_size_def]
+  \\ disch_then (qspec_then ‘(t',t)’ mp_tac) \\ impl_tac >- fs[]
+  \\ rewrite_tac[is_stos_pass_with_plans_correct_def]
+  \\ disch_then (fn ith => last_assum (mp_then Any mp_tac ith))
+  \\ impl_tac \\ fs[]
+  >- (imp_res_tac evaluate_fp_opts_inv \\ fs[])
+  \\ strip_tac \\ pop_assum mp_tac
+  \\ pop_assum (mp_then Any mp_tac (CONJUNCT1 (prep evaluate_fp_rws_up)))
+  \\ disch_then (qspec_then ‘q.fp_state.rws ++ FLAT_h ++ FLAT_plans’ mp_tac) \\ impl_tac
+  >- (fs [SUBSET_DEF] \\ metis_tac[])
+  \\ strip_tac \\ pop_assum (mp_then Any mp_tac (CONJUNCT1 evaluate_add_choices))
+  \\ fs[semState_comp_eq, fpState_component_equality]
+  \\ disch_then (qspec_then ‘choicesR’ assume_tac)
+  \\ first_x_assum (qspec_then ‘fpOpt'’ assume_tac)
+  \\ strip_tac \\ fs[]
+  \\ simp[Once evaluate_cons]
+  \\ qexistsl_tac [‘fpOpt''’, ‘choices’] \\ fs[]
+  \\ fs[semState_comp_eq, fpState_component_equality] \\ conj_tac
+  >- (imp_res_tac evaluate_fp_opts_inv \\ fs[])
+  \\ fs[Once res_sim_cases] \\ fs[v_list_sim_append]
+  \\ irule (CONJUNCT2 res_sim_swap)
+  \\ qexists_tac ‘q’ \\ fs[] \\ imp_res_tac evaluate_fp_opts_inv \\ fs[];
+
+Theorem stos_pass_with_plans_correct_aux:
+  ∀ p.
+    (∀ plan.
+    MEM plan (SND p) ⇒
+      ∀ exps (st1:'a semanticPrimitives$state) st2 env cfg r.
+         is_optimise_with_plan_correct plan st1 st2 env cfg exps r) ⇒
+  ∀ (st1:'a semanticPrimitives$state) st2 env cfg r.
+   is_stos_pass_with_plans_correct (SND p) st1 st2 env cfg (FST p) r
+Proof
+  completeInduct_on ‘(exp6_size (FST p) + LENGTH (SND (p:exp list # opt_step list list)))’
+  \\ strip_tac \\ strip_tac \\ rveq \\ Cases_on ‘p’
+  \\ rename1 ‘SND (exps, plans)’ \\ Cases_on ‘plans’
+  \\ fs[stos_pass_with_plans_correct_empty]
+  \\ rpt strip_tac \\ Cases_on ‘exps’
+  \\ simp[is_stos_pass_with_plans_correct_def, stos_pass_with_plans_def,
+          res_sim_rules, semState_comp_eq, fpState_component_equality,
+          Once stos_pass_with_plans_cons, Once evaluate_append]
+  \\ ntac 4 (TOP_CASE_TAC \\ fs[])
+  \\ rpt strip_tac \\ rveq
+  \\ first_assum (qspec_then ‘h’ mp_tac) \\ impl_tac
+  \\ rewrite_tac[is_optimise_with_plan_correct_def]
+  \\ disch_then (qspec_then ‘[h']’ assume_tac)
+  \\ Cases_on ‘h'’ \\ fs[stos_pass_with_plans_def]
+  \\ qmatch_goalsub_abbrev_tac ‘st1.fp_state with <|
+                                  rws := st1.fp_state.rws ++ FLAT_h ++ FLAT_plans;
+                                  opts := _; choices := _ |>’
+  >~ [‘Fun s e’]
+  >- (
+  fs[MAP_FST_Fun]
+  \\ qpat_x_assum ‘evaluate _ _ [Fun _ _] = _’ mp_tac
+  \\ simp[Once evaluate_def] \\ rpt strip_tac \\ rveq
+  \\ simp[Once evaluate_cons, evaluate_def]
+  \\ first_assum (qspec_then ‘LENGTH t + exp6_size t'’ mp_tac) \\ impl_tac
+  >- (fs[astTheory.exp_size_def])
+  \\ disch_then (qspec_then ‘(t',t)’ mp_tac) \\ simp[]
+  \\ rewrite_tac[is_stos_pass_with_plans_correct_def]
+  \\ disch_then (fn ith => last_assum (mp_then Any mp_tac ith))
+  \\ impl_tac \\ fs[]
+  \\ strip_tac \\ pop_assum mp_tac
+  \\ pop_assum (mp_then Any mp_tac (CONJUNCT1 (prep evaluate_fp_rws_up)))
+  \\ disch_then (qspec_then ‘q.fp_state.rws ++ FLAT_h ++ FLAT_plans’ mp_tac) \\ impl_tac
+  >- (fs [SUBSET_DEF] \\ metis_tac[])
+  \\ rpt strip_tac
+  \\ fs[semState_comp_eq, fpState_component_equality]
+  \\ qexistsl_tac[‘fpOpt'’, ‘choices’]
+  \\ fs[semState_comp_eq, fpState_component_equality] \\ conj_tac
+  >- (imp_res_tac evaluate_fp_opts_inv \\ fs[])
+  \\ ntac 2 (simp [Once res_sim_cases])
+  \\ DISJ2_TAC
+  \\ qexists_tac ‘h’ \\ rpt conj_tac >- fs[]
+  >- (pop_assum mp_tac \\ simp[Once res_sim_cases])
+  \\ rpt strip_tac
+  \\ last_x_assum (qspec_then ‘LENGTH [h] + exp6_size [e]’ mp_tac) \\ impl_tac
+  >- (fs[astTheory.exp_size_def])
+  \\ disch_then (qspec_then ‘([e], [h])’ mp_tac) \\ impl_tac >- fs[]
+  \\ impl_tac
+  >- (last_x_assum (qspec_then ‘h’ mp_tac) \\ fs[])
+  \\ rewrite_tac [is_stos_pass_with_plans_correct_def]
+  \\ rpt (disch_then (fn ith => first_assum $ mp_then Any mp_tac ith))
+  \\ impl_tac \\ fs[]
+  \\ strip_tac \\ qexistsl_tac [‘fpOpt’, ‘choices'’]
+  \\ fs[semState_comp_eq, fpState_component_equality]
+  \\ fs[Once res_sim_cases]
+  \\ irule (CONJUNCT2 res_sim_swap)
+  \\ qexists_tac ‘st’ \\ fs[] \\ imp_res_tac evaluate_fp_opts_inv \\ fs[])
+  >- solve_tac
+  >- solve_tac
+  >- solve_tac
+  >- solve_tac
+  >- solve_tac
+  >- solve_tac
+  >- solve_tac
+  >- solve_tac
+  >- solve_tac
+  >- solve_tac
+  >- solve_tac
+  >- solve_tac
+  >- solve_tac
+  >- solve_tac
+QED
 
 Theorem stos_pass_with_plans_correct:
   ∀ plans.
@@ -2975,70 +3122,72 @@ Theorem stos_pass_with_plans_correct:
   ∀ exps (st1:'a semanticPrimitives$state) st2 env cfg r.
    is_stos_pass_with_plans_correct plans st1 st2 env cfg exps r
 Proof
-  cheat
+  rpt strip_tac
+  \\ qspec_then ‘(exps, plans)’ assume_tac stos_pass_with_plans_correct_aux
+  \\ fs[]
 QED
 
 (* Lemmas needed to automate proof generation *)
 Theorem is_perform_rewrites_correct_empty_plan:
-  ∀ rws path.
-    MEM (Apply (path, rws)) [] ⇒
-    ∀ (st1:'a semanticPrimitives$state) st2 env cfg e r.
-      is_perform_rewrites_correct rws st1 st2 env (cfg with optimisations := rws) e r path
+  ! rws path.
+    MEM (Apply (path, rws)) [] ==>
+    ! (st1:'a semanticPrimitives$state) st2 env cfg e r.
+      is_perform_rewrites_correct rws st1 st2 env cfg e r path
 Proof
   rpt strip_tac \\ fs[]
 QED
 
 Theorem is_perform_rewrites_correct_cons:
-  ∀ rwsNew pathNew plan.
-  (∀ (st1:'a semanticPrimitives$state) st2 env cfg e r.
-      is_perform_rewrites_correct rwsNew st1 st2 env (cfg with optimisations := rwsNew) e r pathNew) ⇒
-  (∀ rws path.
-     MEM (Apply (path, rws)) plan ⇒
-    ∀ (st1:'a semanticPrimitives$state) st2 env cfg e r.
-      is_perform_rewrites_correct rws st1 st2 env (cfg with optimisations := rws) e r path) ⇒
-  (∀ rws path.
-     MEM (Apply (path, rws)) (Apply (pathNew, rwsNew)::plan) ⇒
-    ∀ (st1:'a semanticPrimitives$state) st2 env cfg e r.
-      is_perform_rewrites_correct rws st1 st2 env (cfg with optimisations := rws) e r path)
+  ! rwsNew pathNew plan.
+  (! (st1:'a semanticPrimitives$state) st2 env cfg e r.
+      is_perform_rewrites_correct rwsNew st1 st2 env cfg e r pathNew) ==>
+  (! rws path.
+     MEM (Apply (path, rws)) plan ==>
+    ! (st1:'a semanticPrimitives$state) st2 env cfg e r.
+      is_perform_rewrites_correct rws st1 st2 env cfg e r path) ==>
+  (! rws path.
+     MEM (Apply (path, rws)) (Apply (pathNew, rwsNew)::plan) ==>
+    ! (st1:'a semanticPrimitives$state) st2 env cfg e r.
+      is_perform_rewrites_correct rws st1 st2 env cfg e r path)
 Proof
   rpt strip_tac \\ fs[]
 QED
 
 Theorem is_perform_rewrites_correct_label:
-  ∀ s plan.
-  (∀ rws path.
-     MEM (Apply (path, rws)) plan ⇒
-    ∀ (st1:'a semanticPrimitives$state) st2 env cfg e r.
-      is_perform_rewrites_correct rws st1 st2 env (cfg with optimisations := rws) e r path) ⇒
-  (∀ rws path.
-     MEM (Apply (path, rws)) (Label s::plan) ⇒
-    ∀ (st1:'a semanticPrimitives$state) st2 env cfg e r.
-      is_perform_rewrites_correct rws st1 st2 env (cfg with optimisations := rws) e r path)
+  ! s plan.
+  (! rws path.
+     MEM (Apply (path, rws)) plan ==>
+    ! (st1:'a semanticPrimitives$state) st2 env cfg e r.
+      is_perform_rewrites_correct rws st1 st2 env cfg e r path) ==>
+  (! rws path.
+     MEM (Apply (path, rws)) (Label s::plan) ==>
+    ! (st1:'a semanticPrimitives$state) st2 env cfg e r.
+      is_perform_rewrites_correct rws st1 st2 env cfg e r path)
 Proof
   rpt strip_tac \\ fs[]
 QED
 
 Theorem is_perform_rewrites_correct_expected:
-  ∀ e plan.
-  (∀ rws path.
-     MEM (Apply (path, rws)) plan ⇒
-    ∀ (st1:'a semanticPrimitives$state) st2 env cfg e r.
-      is_perform_rewrites_correct rws st1 st2 env (cfg with optimisations := rws) e r path) ⇒
-  (∀ rws path.
-     MEM (Apply (path, rws)) (Expected e::plan) ⇒
-    ∀ (st1:'a semanticPrimitives$state) st2 env cfg e r.
-      is_perform_rewrites_correct rws st1 st2 env (cfg with optimisations := rws) e r path)
+  ! e plan.
+  (! rws path.
+     MEM (Apply (path, rws)) plan ==>
+    ! (st1:'a semanticPrimitives$state) st2 env cfg e r.
+      is_perform_rewrites_correct rws st1 st2 env cfg e r path) ==>
+  (! rws path.
+     MEM (Apply (path, rws)) (Expected e::plan) ==>
+    ! (st1:'a semanticPrimitives$state) st2 env cfg e r.
+      is_perform_rewrites_correct rws st1 st2 env cfg e r path)
 Proof
   rpt strip_tac \\ fs[]
 QED
 
 Theorem is_optimise_with_plan_correct_sing:
-  ∀ sing_plan.
-    (∀ (st1:'a semanticPrimitives$state) st2 env cfg exps r.
-    is_optimise_with_plan_correct sing_plan st1 st2 env cfg exps r) ⇒
-    (∀ plan.
-       MEM plan [sing_plan] ⇒
-       ∀ exps (st1:'a semanticPrimitives$state) st2 env cfg r.
+  ! sing_plan.
+    (! (st1:'a semanticPrimitives$state) st2 env cfg exps r.
+    is_optimise_with_plan_correct sing_plan st1 st2 env cfg exps r) ==>
+    (! plan.
+       MEM plan [sing_plan] ==>
+       ! exps (st1:'a semanticPrimitives$state) st2 env cfg r.
        is_optimise_with_plan_correct plan st1 st2 env cfg exps r)
 Proof
   rpt strip_tac \\ fs[]
@@ -3076,9 +3225,9 @@ local
    \\ rpt conj_tac \\ imp_res_tac evaluate_fp_opts_inv \\ fs[];
 in
 Theorem stos_pass_correct:
-  ∀ exps (st1:'a semanticPrimitives$state) st2 env cfg r.
-  (∀ exps (st1:'a semanticPrimitives$state) st2 env cfg r.
-    is_optimise_correct rws st1 st2 env cfg exps r) ⇒
+  ! exps (st1:'a semanticPrimitives$state) st2 env cfg r.
+  (! exps (st1:'a semanticPrimitives$state) st2 env cfg r.
+    is_optimise_correct rws st1 st2 env cfg exps r) ==>
    is_stos_pass_correct rws st1 st2 env cfg exps r
 Proof
   measureInduct_on ‘exp6_size exps’ \\ fs[is_stos_pass_correct_def]
@@ -3087,7 +3236,7 @@ Proof
   >- (rveq \\ fs[res_sim_rules])
   \\ qpat_x_assum `evaluate _ _ _ = _` mp_tac
   \\ simp[Once evaluate_cons, Once evaluate_append]
-  \\ Cases_on ‘evaluate st1 env (stos_pass (cfg with optimisations := rws) [h])’
+  \\ Cases_on ‘evaluate st1 env (stos_pass cfg [h])’
   \\ Cases_on ‘h’ \\ fs[stos_pass_def]
   >- optimise_case ‘[Raise e]’
   >- optimise_case ‘[Handle e l]’
@@ -3142,11 +3291,11 @@ val _ = export_theory ();
 Definition is_optimise_correct_def:
   is_optimise_correct rws (st1:'a semanticPrimitives$state) st2 env cfg exps r =
     (evaluate st1 env
-             (MAP (optimise (cfg with optimisations := rws)) exps) = (st2, Rval r) ∧
-    (cfg.canOpt ⇔ st1.fp_state.canOpt = FPScope Opt) ∧
-    st1.fp_state.canOpt ≠ Strict ∧
+             (MAP (optimise cfg) exps) = (st2, Rval r) /\
+    (cfg.canOpt <=> st1.fp_state.canOpt = FPScope Opt) /\
+    st1.fp_state.canOpt <> Strict /\
     (~ st1.fp_state.real_sem) ==>
-    ∃ fpOpt choices fpOptR choicesR.
+    ? fpOpt choices fpOptR choicesR.
       evaluate (st1 with fp_state := st1.fp_state with
                 <| rws := st1.fp_state.rws ++ rws; opts := fpOpt; choices := choices |>) env exps =
         (st2 with fp_state := st2.fp_state with
@@ -3165,7 +3314,7 @@ QED
 
 (*
 Theorem optimise_empty_sing:
-  ∀ cfg e. optimise (cfg with optimisations := []) e = e
+  ! cfg e. optimise (cfg with optimisations := []) e = e
 Proof
   ho_match_mp_tac optimise_ind
   \\ rpt strip_tac \\ fs[optimise_def]
@@ -3198,7 +3347,7 @@ QED *)
 
 (*
 Theorem optimise_empty:
-  ∀ exps cfg. MAP (optimise (cfg with optimisations := [])) exps = exps
+  ! exps cfg. MAP (optimise (cfg with optimisations := [])) exps = exps
 Proof
   Induct_on ‘exps’ \\ rpt strip_tac
   >- (EVAL_TAC)
@@ -3208,7 +3357,7 @@ QED
 
 (*
 Theorem optimise_pat_empty:
-  ∀ pl cfg. MAP (λ (p,e). (p, optimise (cfg with optimisations := []) e)) pl = pl
+  ! pl cfg. MAP (λ (p,e). (p, optimise (cfg with optimisations := []) e)) pl = pl
 Proof
   Induct_on ‘pl’ \\ rpt strip_tac >- (EVAL_TAC)
   \\ fs[] \\ Cases_on ‘h’ \\ fs[optimise_empty_sing]
@@ -3221,14 +3370,14 @@ local
   (* exp goal *)
   val P0 =
   “λ (e:ast$exp).
-     ∀ (st1: 'a semanticPrimitives$state) st2 env cfg rws r.
-     (∀ (st1:'a semanticPrimitives$state) st2 env exps r.
-       is_rewriteFPexp_list_correct rws st1 st2 env exps r) ∧
-     (cfg.canOpt ⇔ st1.fp_state.canOpt = FPScope Opt) ∧
-     st1.fp_state.canOpt ≠ Strict ∧
-     ~st1.fp_state.real_sem ∧
-     evaluate st1 env [optimise (cfg with optimisations := rws) e] = (st2, Rval r) ⇒
-    ∃ fpOpt choices fpOptR choicesR.
+     ! (st1: 'a semanticPrimitives$state) st2 env cfg rws r.
+     (! (st1:'a semanticPrimitives$state) st2 env exps r.
+       is_rewriteFPexp_list_correct rws st1 st2 env exps r) /\
+     (cfg.canOpt <=> st1.fp_state.canOpt = FPScope Opt) /\
+     st1.fp_state.canOpt <> Strict /\
+     ~st1.fp_state.real_sem /\
+     evaluate st1 env [optimise cfg e] = (st2, Rval r) ==>
+    ? fpOpt choices fpOptR choicesR.
       evaluate (st1 with fp_state := st1.fp_state with
                 <| rws := st1.fp_state.rws ++ rws; opts := fpOpt; choices := choices |>) env [e]=
         (st2 with fp_state := st2.fp_state with
@@ -3242,21 +3391,21 @@ local
   (* Letrec goal *)
   val P1 =
   Parse.Term (‘λ (l:(string # string # exp) list).
-  ∀ p. MEM p l ⇒ ^P2 p’)
+  ! p. MEM p l ==> ^P2 p’)
   (* P5: pat * exp -> bool *)
   val P5 =
   Parse.Term (‘λ (p:pat, e). ^P0 e’)
   (* P3: pat * exp list -> bool *)
   val P3 =
   Parse.Term (‘λ (l:(pat # exp) list).
-     ∀ (st1: 'a semanticPrimitives$state) st2 env cfg rws r v err_v.
-     (∀ (st1:'a semanticPrimitives$state) st2 env exps r.
-       is_rewriteFPexp_list_correct rws st1 st2 env exps r) ∧
-     (cfg.canOpt ⇔ st1.fp_state.canOpt = FPScope Opt) ∧
-     st1.fp_state.canOpt ≠ Strict ∧
-     ~st1.fp_state.real_sem ∧
-     evaluate_match st1 env v (MAP (λ (p,e). (p, optimise (cfg with optimisations := rws) e)) l) err_v = (st2, Rval r) ⇒
-     ∃ fpOpt choices fpOptR choicesR.
+     ! (st1: 'a semanticPrimitives$state) st2 env cfg rws r v err_v.
+     (! (st1:'a semanticPrimitives$state) st2 env exps r.
+       is_rewriteFPexp_list_correct rws st1 st2 env exps r) /\
+     (cfg.canOpt <=> st1.fp_state.canOpt = FPScope Opt) /\
+     st1.fp_state.canOpt <> Strict /\
+     ~st1.fp_state.real_sem /\
+     evaluate_match st1 env v (MAP (λ (p,e). (p, optimise cfg e)) l) err_v = (st2, Rval r) ==>
+     ? fpOpt choices fpOptR choicesR.
        evaluate_match
          (st1 with fp_state := st1.fp_state with <| rws := st1.fp_state.rws ++ rws; opts := fpOpt; choices := choices |>)
          env v l err_v =
@@ -3264,7 +3413,7 @@ local
            <| rws := st2.fp_state.rws ++ rws; opts := fpOptR; choices := choicesR |>, Rval r)’);
   (* P6: exp list -> bool *)
   val P6 =
-    Parse.Term (‘λ (es:ast$exp list). ∀ e. MEM e es ⇒ ^P0 e’);
+    Parse.Term (‘λ (es:ast$exp list). ! e. MEM e es ==> ^P0 e’);
   val ind_thm =
     astTheory.exp_induction |> SPEC P0 |> SPEC P1 |> SPEC P2 |> SPEC P3
     |> SPEC P4 |> SPEC P5 |> SPEC P6;
@@ -3288,16 +3437,16 @@ local
 in
 
 Triviality lift_P6_REVERSE:
-  ∀ es.
-    ^P6 es ⇒
-    ∀ (st1: 'a semanticPrimitives$state) st2 env cfg rws r.
-    (∀ (st1:'a semanticPrimitives$state) st2 env exps r.
-      is_rewriteFPexp_list_correct rws st1 st2 env exps r) ∧
-    (cfg.canOpt ⇔ st1.fp_state.canOpt = FPScope Opt) ∧
-    st1.fp_state.canOpt ≠ Strict ∧
-    ~st1.fp_state.real_sem ∧
-    evaluate st1 env (MAP (λ e. optimise (cfg with optimisations := rws) e) (REVERSE es)) = (st2, Rval r) ⇒
-    ∃ fpOpt choices fpOptR choicesR.
+  ! es.
+    ^P6 es ==>
+    ! (st1: 'a semanticPrimitives$state) st2 env cfg rws r.
+    (! (st1:'a semanticPrimitives$state) st2 env exps r.
+      is_rewriteFPexp_list_correct rws st1 st2 env exps r) /\
+    (cfg.canOpt <=> st1.fp_state.canOpt = FPScope Opt) /\
+    st1.fp_state.canOpt <> Strict /\
+    ~st1.fp_state.real_sem /\
+    evaluate st1 env (MAP (λ e. optimise cfg e) (REVERSE es)) = (st2, Rval r) ==>
+    ? fpOpt choices fpOptR choicesR.
       evaluate
         (st1 with fp_state := st1.fp_state with <| rws := st1.fp_state.rws ++ rws; opts := fpOpt; choices := choices |>)
         env (REVERSE es) =
@@ -3313,7 +3462,7 @@ Proof
   \\ get_ext_eval_tac ‘evaluate st1 env (MAP _ _) = _’
   \\ pop_assum mp_tac \\ impl_tac
   >- (rpt strip_tac \\ fs[]
-      \\ qpat_x_assum ‘∀ e. (e = h ∨ MEM e es) ⇒ _’ mp_tac
+      \\ qpat_x_assum ‘! e. (e = h \/ MEM e es) ==> _’ mp_tac
       \\ disch_then (qspec_then ‘e’ mp_tac) \\ impl_tac \\ fs[]
       \\ rpt (disch_then drule) \\ strip_tac
       \\ qexists_tac ‘fpOpt’ \\ qexists_tac ‘choices’
@@ -3322,8 +3471,8 @@ Proof
   \\ rpt (TOP_CASE_TAC \\ fs[])
   \\ rpt strip_tac \\ rveq
   \\ first_x_assum (qspec_then ‘h’ mp_tac) \\ fs[] \\ rveq
-  \\ ‘(cfg.canOpt ⇔ q.fp_state.canOpt = FPScope Opt) ∧
-      q.fp_state.canOpt ≠ Strict ∧ ~ q.fp_state.real_sem’
+  \\ ‘(cfg.canOpt <=> q.fp_state.canOpt = FPScope Opt) /\
+      q.fp_state.canOpt <> Strict /\ ~ q.fp_state.real_sem’
     by (imp_res_tac evaluate_fp_opts_inv \\ fs[])
   \\ rpt (disch_then drule) \\ strip_tac
   \\ optUntil_tac ‘evaluate _ _ (REVERSE es) = _’ ‘fpOpt'’
@@ -3336,16 +3485,16 @@ Proof
 QED
 
 Triviality lift_P6:
-  ∀ es.
-    ^P6 es ⇒
-    ∀ (st1: 'a semanticPrimitives$state) st2 env cfg rws r.
-    (∀ (st1:'a semanticPrimitives$state) st2 env exps r.
-      is_rewriteFPexp_list_correct rws st1 st2 env exps r) ∧
-    (cfg.canOpt ⇔ st1.fp_state.canOpt = FPScope Opt) ∧
-    st1.fp_state.canOpt ≠ Strict ∧
-    ~st1.fp_state.real_sem ∧
-    evaluate st1 env (MAP (λ e. optimise (cfg with optimisations := rws) e) es) = (st2, Rval r) ⇒
-    ∃ fpOpt choices fpOptR choicesR.
+  ! es.
+    ^P6 es ==>
+    ! (st1: 'a semanticPrimitives$state) st2 env cfg rws r.
+    (! (st1:'a semanticPrimitives$state) st2 env exps r.
+      is_rewriteFPexp_list_correct rws st1 st2 env exps r) /\
+    (cfg.canOpt <=> st1.fp_state.canOpt = FPScope Opt) /\
+    st1.fp_state.canOpt <> Strict /\
+    ~st1.fp_state.real_sem /\
+    evaluate st1 env (MAP (λ e. optimise cfg e) es) = (st2, Rval r) ==>
+    ? fpOpt choices fpOptR choicesR.
       evaluate
         (st1 with fp_state := st1.fp_state with <| rws := st1.fp_state.rws ++ rws; opts := fpOpt; choices := choices |>)
         env es =
@@ -3367,7 +3516,7 @@ Proof
   \\ last_x_assum mp_tac  \\ impl_tac
   >- (
    rpt strip_tac \\ fs[]
-   \\ qpat_x_assum ‘∀ e. (e = h ∨ MEM e es) ⇒ _’ mp_tac
+   \\ qpat_x_assum ‘! e. (e = h \/ MEM e es) ==> _’ mp_tac
    \\ disch_then (qspec_then ‘e’ mp_tac) \\ impl_tac \\ fs[]
    \\ rpt (disch_then drule) \\ strip_tac
    \\ qexists_tac ‘fpOpt'’ \\ qexists_tac ‘choices'’
@@ -3386,8 +3535,8 @@ Proof
 QED
 
 Theorem optimise_correct:
-  (∀ e. ^P0 e) ∧ (∀ l. ^P1 l) ∧ (∀ p. ^P2 p) ∧ (∀ l. ^P3 l) ∧ (∀ p. ^P4 p)
-  ∧ (∀ p. ^P5 p) ∧ (∀ l. ^P6 l)
+  (! e. ^P0 e) /\ (! l. ^P1 l) /\ (! p. ^P2 p) /\ (! l. ^P3 l) /\ (! p. ^P4 p)
+  /\ (! p. ^P5 p) /\ (! l. ^P6 l)
 Proof
   irule ind_thm \\ rpt strip_tac \\ fs[optimise_def] \\ rpt strip_tac
   \\ TRY (qpat_x_assum `evaluate _ _ _ = _` mp_tac)
@@ -3401,8 +3550,8 @@ Proof
    \\ Cases_on ‘v = Boolv T’ \\ fs[]
    >- (
     strip_tac
-    \\ ‘(cfg.canOpt ⇔ q.fp_state.canOpt = FPScope Opt) ∧
-        q.fp_state.canOpt ≠ Strict ∧ ~ q.fp_state.real_sem’
+    \\ ‘(cfg.canOpt <=> q.fp_state.canOpt = FPScope Opt) /\
+        q.fp_state.canOpt <> Strict /\ ~ q.fp_state.real_sem’
        by (imp_res_tac evaluate_fp_opts_inv \\ fs[])
     \\ last_x_assum drule
     \\ rpt (disch_then drule)
@@ -3415,8 +3564,8 @@ Proof
     \\ fs[semState_comp_eq, fpState_component_equality])
    \\ Cases_on ‘v = Boolv F’ \\ fs[]
    \\ strip_tac
-   \\ ‘(cfg.canOpt ⇔ q.fp_state.canOpt = FPScope Opt) ∧
-       q.fp_state.canOpt ≠ Strict ∧ ~ q.fp_state.real_sem’
+   \\ ‘(cfg.canOpt <=> q.fp_state.canOpt = FPScope Opt) /\
+       q.fp_state.canOpt <> Strict /\ ~ q.fp_state.real_sem’
      by (imp_res_tac evaluate_fp_opts_inv \\ fs[])
    \\ first_x_assum drule
    \\ rpt (disch_then drule)
@@ -3432,14 +3581,14 @@ Proof
    \\ ntac 2 (reverse TOP_CASE_TAC \\ fs[])
    \\ get_ext_eval_tac ‘evaluate st1 _ [optimise _ e] = _’
    \\ fs[do_log_def]
-   \\ Cases_on ‘l = And ∧ HD a = Boolv T ∨ l = Or ∧ HD a = Boolv F’ \\ fs[]
+   \\ Cases_on ‘l = And /\ HD a = Boolv T \/ l = Or /\ HD a = Boolv F’ \\ fs[]
    \\ rveq \\ fs[]
    \\ TRY (
       rpt strip_tac
       \\ qpat_x_assum `evaluate q env [optimise _ e0] = _`
                       (fn th => first_x_assum (fn ith => mp_then Any mp_tac ith th))
-      \\ ‘(cfg.canOpt ⇔ q.fp_state.canOpt = FPScope Opt) ∧
-          q.fp_state.canOpt ≠ Strict ∧ ~ q.fp_state.real_sem’
+      \\ ‘(cfg.canOpt <=> q.fp_state.canOpt = FPScope Opt) /\
+          q.fp_state.canOpt <> Strict /\ ~ q.fp_state.real_sem’
         by (imp_res_tac evaluate_fp_opts_inv \\ fs[])
       \\ rfs[]
       \\ rpt (disch_then drule)
@@ -3451,7 +3600,7 @@ Proof
       \\ rpt (qpat_x_assum ‘evaluate _ _ _ = _’ (mp_then Any mp_tac (CONJUNCT1 evaluate_add_choices)))
       \\ rpt (disch_then (qspec_then ‘choicesR’ assume_tac))
       \\ fs[semState_comp_eq, fpState_component_equality])
-   \\ Cases_on ‘l = Or ∧ HD a = Boolv T’ \\ Cases_on ‘l = And ∧ HD a = Boolv F’
+   \\ Cases_on ‘l = Or /\ HD a = Boolv T’ \\ Cases_on ‘l = And /\ HD a = Boolv F’
    \\ fs[]
    \\ rpt strip_tac \\ rveq \\ qexists_tac ‘fpOpt’ \\ qexists_tac ‘choices’
    \\ fs[] \\ fs[semState_comp_eq, fpState_component_equality])
@@ -3460,8 +3609,8 @@ Proof
    \\ ntac 2 (reverse TOP_CASE_TAC \\ fs[])
    \\ get_ext_eval_tac ‘evaluate st1 env [optimise _ e] = _’
    \\ strip_tac
-   \\ ‘(cfg.canOpt ⇔ q.fp_state.canOpt = FPScope Opt) ∧
-        q.fp_state.canOpt ≠ Strict ∧ ~ q.fp_state.real_sem’
+   \\ ‘(cfg.canOpt <=> q.fp_state.canOpt = FPScope Opt) /\
+        q.fp_state.canOpt <> Strict /\ ~ q.fp_state.real_sem’
       by (imp_res_tac evaluate_fp_opts_inv \\ fs[])
    \\ first_x_assum drule \\ rpt (disch_then drule)
    \\ strip_tac
@@ -3496,8 +3645,8 @@ Proof
    \\ TOP_CASE_TAC \\ fs[]
    \\ get_ext_eval_tac ‘evaluate st1 env [optimise _ e] = _’
    \\ strip_tac
-   \\ ‘(cfg.canOpt ⇔ q.fp_state.canOpt = FPScope Opt) ∧
-        q.fp_state.canOpt ≠ Strict ∧ ~ q.fp_state.real_sem’
+   \\ ‘(cfg.canOpt <=> q.fp_state.canOpt = FPScope Opt) /\
+        q.fp_state.canOpt <> Strict /\ ~ q.fp_state.real_sem’
       by (imp_res_tac evaluate_fp_opts_inv \\ fs[])
    \\ first_x_assum drule \\ rpt (disch_then drule)
    \\ strip_tac
@@ -3516,12 +3665,12 @@ Proof
    \\ ntac 2 (reverse TOP_CASE_TAC \\ fs[])
    \\ rpt strip_tac \\ rveq \\ fs[]
    \\ fs[]
-   \\ ‘<| optimisations := rws; canOpt := (f = Opt) |>.canOpt ⇔
+   \\ ‘<| optimisations := rws; canOpt := (f = Opt) |>.canOpt <=>
        (st1 with fp_state := st1.fp_state with canOpt := FPScope f).fp_state.canOpt = FPScope Opt’
      by (Cases_on ‘f’ \\ fs[semState_comp_eq, fpState_component_equality])
    \\ ‘~ (st1 with fp_state := st1.fp_state with canOpt := FPScope f).fp_state.real_sem’
         by (fs[semState_comp_eq, fpState_component_equality])
-   \\ ‘(st1 with fp_state := st1.fp_state with canOpt := FPScope f).fp_state.canOpt ≠ Strict’
+   \\ ‘(st1 with fp_state := st1.fp_state with canOpt := FPScope f).fp_state.canOpt <> Strict’
         by (fs[semState_comp_eq, fpState_component_equality])
    \\ first_x_assum drule \\ rpt (disch_then drule)
    \\ disch_then (qspecl_then [‘q’, ‘env’, ‘a’] mp_tac)
@@ -3553,11 +3702,11 @@ Proof
    \\ rpt strip_tac \\ rveq
    \\ fs[semState_comp_eq, fpState_component_equality])
   >- (
-   qpat_x_assum ‘∀ e. MEM e l ⇒ _’
+   qpat_x_assum ‘! e. MEM e l ==> _’
      (fn thm => (mp_then Any assume_tac (SIMP_RULE std_ss [] lift_P6_REVERSE) thm))
    \\ Cases_on ‘st1.fp_state.canOpt = FPScope Opt’ \\ fs[]
    >- (
-    qpat_assum ‘∀ st1 st2 env exps r.
+    qpat_assum ‘! st1 st2 env exps r.
                 is_rewriteFPexp_list_correct rws st1 st2 env _ _’ mp_tac
     \\ once_rewrite_tac[is_rewriteFPexp_list_correct_def]
     \\ rpt strip_tac
@@ -3566,15 +3715,15 @@ Proof
     \\ first_x_assum
        (qspecl_then
         [‘st1’, ‘st2’, ‘env’,
-         ‘[App o' (MAP (λ a. optimise (cfg with optimisations := rws) a )l)]’, ‘r’]
+         ‘[App o' (MAP (λ a. optimise cfg a )l)]’, ‘r’]
         mp_tac)
     \\ impl_tac \\ fs[]
     \\ qpat_x_assum `evaluate _ _ [rewriteFPexp _ _ ] = _` kall_tac
     \\ rpt strip_tac
     \\ qpat_x_assum `evaluate _ _ _ = _` mp_tac
     \\ qmatch_goalsub_abbrev_tac ‘evaluate st1_ext env _’
-    \\ ‘(cfg.canOpt ⇔ st1_ext.fp_state.canOpt = FPScope Opt) ∧
-        st1_ext.fp_state.canOpt ≠ Strict ∧ ~ st1_ext.fp_state.real_sem’
+    \\ ‘(cfg.canOpt <=> st1_ext.fp_state.canOpt = FPScope Opt) /\
+        st1_ext.fp_state.canOpt <> Strict /\ ~ st1_ext.fp_state.real_sem’
        by (unabbrev_all_tac \\ fs[semState_comp_eq, fpState_component_equality])
     \\ disch_then (fn thm => mp_tac (REWRITE_RULE [Once evaluate_def] thm))
     \\ ntac 2 (reverse TOP_CASE_TAC \\ fs[])
@@ -3622,7 +3771,7 @@ Proof
      \\ rpt strip_tac \\ rveq \\ fs[shift_fp_opts_def]
      \\ optUntil_tac ‘evaluate _ _ (REVERSE _) = _’ ‘q.fp_state.opts’
      \\ rfs[fpState_component_equality]
-     \\ qexists_tac ‘optUntil (choicesR' − choices') fpOpt'' q.fp_state.opts’
+     \\ qexists_tac ‘optUntil (choicesR' - choices') fpOpt'' q.fp_state.opts’
      \\ qexists_tac ‘choices'’
      \\ simp[evaluate_def]
      \\ fs[] \\ TOP_CASE_TAC
@@ -3671,7 +3820,7 @@ Proof
      \\ rveq \\ rfs[]
      \\ fs[semState_comp_eq, fpState_component_equality])
     >- (
-     ‘q.fp_state.canOpt ≠ FPScope Opt’ by (imp_res_tac evaluate_fp_opts_inv \\ fs[])
+     ‘q.fp_state.canOpt <> FPScope Opt’ by (imp_res_tac evaluate_fp_opts_inv \\ fs[])
      \\ fs[]
      \\ ntac 3 (TOP_CASE_TAC \\ fs[])
      \\ rpt strip_tac \\ rveq \\ simp[evaluate_def]
@@ -3682,7 +3831,7 @@ Proof
     \\ ‘~q.fp_state.real_sem’ by (imp_res_tac evaluate_fp_opts_inv \\ fs[])
     \\ fs[shift_fp_opts_def])
   >- (
-   qpat_x_assum ‘∀ e. MEM e l ⇒ _’
+   qpat_x_assum ‘! e. MEM e l ==> _’
      (fn thm => (mp_then Any assume_tac (SIMP_RULE std_ss [] lift_P6_REVERSE) thm))
    \\ simp [evaluate_def]
    \\ reverse TOP_CASE_TAC \\ fs[]
@@ -3725,20 +3874,20 @@ end;
 Definition is_stos_pass_correct_def :
   is_stos_pass_correct rws (st1:'a semanticPrimitives$state) st2 env cfg exps r1 =
     (evaluate st1 env
-             (stos_pass (cfg with optimisations := rws) exps) = (st2, Rval r1) ∧
-     (cfg.canOpt ⇔ st1.fp_state.canOpt = FPScope Opt) ∧
-     (st1.fp_state.canOpt ≠ Strict) ∧
+             (stos_pass cfg exps) = (st2, Rval r1) /\
+     (cfg.canOpt <=> st1.fp_state.canOpt = FPScope Opt) /\
+     (st1.fp_state.canOpt <> Strict) /\
      (~ st1.fp_state.real_sem) ==>
-    ∃ fpOpt choices fpOptR choicesR r2.
+    ? fpOpt choices fpOptR choicesR r2.
       (evaluate (st1 with fp_state := st1.fp_state with
                 <| rws := st1.fp_state.rws ++ rws; opts := fpOpt; choices := choices |>) env exps =
       (st2 with fp_state := st2.fp_state with
-       <| rws := st2.fp_state.rws ++ rws; opts := fpOptR; choices := choicesR |>, Rval r2)) ∧
-      res_sim (Rval r1) (Rval r2) (cfg with optimisations := rws) st1)
+       <| rws := st2.fp_state.rws ++ rws; opts := fpOptR; choices := choicesR |>, Rval r2)) /\
+      res_sim (Rval r1) (Rval r2) cfg st1)
 End
 
 Theorem optimise_with_plan_let:
-  ∀cfg plan sc e1 e2 x a. optimise_with_plan cfg plan (Let a e1 e2) = x ⇒ ∃e1' e2'. x = (Let a e1' e2')
+  !cfg plan sc e1 e2 x a. optimise_with_plan cfg plan (Let a e1 e2) = x ==> ?e1' e2'. x = (Let a e1' e2')
 Proof
   Induct_on ‘plan’
   >- fs[optimise_with_plan_empty_sing]
@@ -3748,19 +3897,19 @@ Proof
   \\ fs[optimise_with_plan_def]
   \\ Cases_on ‘h0’ \\ fs[perform_rewrites_def]
   \\ TRY (
-    qpat_x_assum ‘∀ cfg' e1' e2' a. ∃ e1'' e2''. optimise_with_plan _ _ _ = _’ (
+    qpat_x_assum ‘! cfg' e1' e2' a. ? e1'' e2''. optimise_with_plan _ _ _ = _’ (
                    qspecl_then [‘cfg’, ‘perform_rewrites (cfg with optimisations := h1) o' h1 e1’, ‘e2’, ‘a’] strip_assume_tac
                    )
     \\ qexists_tac ‘e1'’ \\ qexists_tac ‘e2'’ \\ fs[] \\ NO_TAC
     )
   \\ TRY (
-    qpat_x_assum ‘∀ cfg' e1' e2' a. ∃ e1'' e2''. optimise_with_plan _ _ _ = _’ (
+    qpat_x_assum ‘! cfg' e1' e2' a. ? e1'' e2''. optimise_with_plan _ _ _ = _’ (
                    qspecl_then [‘cfg’, ‘e1’, ‘perform_rewrites (cfg with optimisations := h1) o' h1 e2’, ‘a’] strip_assume_tac
                    )
     \\ qexists_tac ‘e1'’ \\ qexists_tac ‘e2'’ \\ fs[] \\ NO_TAC
     )
   \\ TRY (
-    qpat_x_assum ‘∀ cfg' e1' e2' a. ∃ e1'' e2''. optimise_with_plan _ _ _ = _’ (
+    qpat_x_assum ‘! cfg' e1' e2' a. ? e1'' e2''. optimise_with_plan _ _ _ = _’ (
                    qspecl_then [‘cfg’, ‘e1’, ‘e2’, ‘a’] strip_assume_tac
                    )
     \\ qexists_tac ‘e1'’ \\ qexists_tac ‘e2'’ \\ fs[] \\ NO_TAC
@@ -3797,9 +3946,9 @@ Proof
 QED
 
 Theorem stos_pass_with_plans_empty[simp]:
-  ∀ cfg es. stos_pass_with_plans cfg [] es = es
+  ! cfg es. stos_pass_with_plans cfg [] es = es
 Proof
-  qspec_then ‘λ cfg plans es. plans = [] ⇒ stos_pass_with_plans cfg plans es = es’
+  qspec_then ‘λ cfg plans es. plans = [] ==> stos_pass_with_plans cfg plans es = es’
          mp_tac stos_pass_with_plans_ind
   \\ impl_tac \\ rpt strip_tac \\ fs[stos_pass_with_plans_def]
 QED
@@ -3847,9 +3996,9 @@ QED
 
 (*
 Theorem is_optimise_correct_lift:
-  (∀ (st1:'a semanticPrimitives$state) st2 env exps r.
-    is_rewriteFPexp_list_correct rws st1 st2 env exps r) ⇒
-  (∀ (st1:'a semanticPrimitives$state) st2 env cfg exps r.
+  (! (st1:'a semanticPrimitives$state) st2 env exps r.
+    is_rewriteFPexp_list_correct rws st1 st2 env exps r) ==>
+  (! (st1:'a semanticPrimitives$state) st2 env cfg exps r.
     is_optimise_correct rws st1 st2 env cfg exps r)
 Proof
   rpt strip_tac
@@ -3864,7 +4013,7 @@ Proof
   \\ impl_tac
   >- (
    rpt conj_tac \\ fs[]
-   \\ ‘(λ e. optimise (cfg with optimisations := rws) e) = optimise (cfg with optimisations := rws) ’
+   \\ ‘(λ e. optimise cfg e) = optimise cfg ’
      by (fs[FUN_EQ_THM])
    \\ pop_assum (fs o single))
   \\ rpt strip_tac \\ fsrw_tac [SATISFY_ss] []
